@prefix : <http://data.odeuropa.eu/ontology#> .
@prefix od: <http://data.odeuropa.eu/ontology/> .
@prefix crm: <http://erlangen-crm.org/current/> .
@prefix owl: <http://www.w3.org/2002/07/owl#> .
@prefix rdf: <http://www.w3.org/1999/02/22-rdf-syntax-ns#> .
@prefix xml: <http://www.w3.org/XML/1998/namespace> .
@prefix xsd: <http://www.w3.org/2001/XMLSchema#> .
@prefix rdfs: <http://www.w3.org/2000/01/rdf-schema#> .
@prefix vann: <http://purl.org/vocab/vann/> .
@prefix crmsci: <http://www.ics.forth.gr/isl/CRMsci/> .

<http://data.odeuropa.eu/ontology/> rdf:type owl:Ontology ;
                                     owl:imports crm: ;
                                     vann:preferredNamespaceUri "http://data.odeuropa.eu/ontology/" ;
                                     dc:creator <http://data.odeuropa.eu/odeuropa>;
                                     owl:versionInfo "0.2" .

#################################################################
#    Object Properties
#################################################################

###  http://data.odeuropa.eu/ontology/F10_targeted
od:F10_targeted rdf:type owl:ObjectProperty ;
                rdfs:subPropertyOf crm:P16_used_specific_object ;
                rdfs:domain od:L16_Odorizing ;
                rdfs:comment """This property associates an instance of L16 Odorizing with the thing to which the smell was applyed.

Examples:
* A woman uses a perfume on her body
* A perfume was sprayed in the whole apartment"""@en .


###  http://data.odeuropa.eu/ontology/F1_generated
od:F1_generated rdf:type owl:ObjectProperty ;
                rdfs:subPropertyOf crm:P92_brought_into_existence ;
                rdf:type owl:AsymmetricProperty ;
                rdfs:domain od:L2_Stimulus_Generation ;
                rdfs:range od:L1_Sensory_Stimulus ;
                rdfs:comment "This property associates an instance of L2 Stimulus Generation with the L1 Sensory Stimulus which was created by the event."@en ;
                owl:cardinality "1"^^xsd:nonNegativeInteger .


###  http://data.odeuropa.eu/ontology/F2_perceived
od:F2_perceived rdf:type owl:ObjectProperty ;
                rdfs:subPropertyOf crmsci:O8_observed ;
                rdf:type owl:AsymmetricProperty ;
                rdfs:domain od:L3_Sensory_Experience ;
                rdfs:range od:L1_Sensory_Stimulus ;
                rdfs:comment "This property associates an instance of L3 Sensory Experience with the L1 Sensory Stimulus which was experienced."@en ;
                owl:cardinality "1"^^xsd:nonNegativeInteger .


###  http://data.odeuropa.eu/ontology/F3_had_source
od:F3_had_source rdf:type owl:ObjectProperty ;
                 rdfs:subPropertyOf crm:P12_occurred_in_the_presence_of ;
                 rdfs:domain od:L2_Stimulus_Generation ;
                 rdfs:range crmsci:S10_Material_Substantial ;
                 rdfs:comment """This property associates an instance of L2 Stimulus Generation with the S10 Material Substantial which generate the stimulus.

Examples:
* The played violin (stimulus: sound)
* An ice-cream (stimulus: taste)
* A perfumed candle (stimulus: smell)"""@en .


###  http://data.odeuropa.eu/ontology/F4_had_carrier
od:F4_had_carrier rdf:type owl:ObjectProperty ;
                  rdfs:subPropertyOf crm:P12_occurred_in_the_presence_of ;
                  rdfs:domain od:L2_Stimulus_Generation ;
                  rdfs:range crmsci:S10_Material_Substantial ;
                  rdfs:comment """This property associates an instance of L2 Stimulus Generation with the object that it is not directly emitting the stimulus, but rather carrying it.

Examples:
* A pipe (stimulus: smell of tobacco)
* The bell tower (stimulus: sound of the bell)"""@en .


###  http://data.odeuropa.eu/ontology/F5_involved_gesture
od:F5_involved_gesture rdf:type owl:ObjectProperty ;
                       rdfs:subPropertyOf crm:P9_consists_of ;
                       rdfs:domain crm:E7_Activity ;
                       rdfs:range od:L7_Gesture ;
                       rdfs:comment """This property associates an instance of E7 Activity with an L7 Gesture happening contextually.

Examples:
* During the meeting, I was yawning all the time
* When perceiving that smell, I had to cover my nose"""@en .


###  http://data.odeuropa.eu/ontology/F6_evoked
od:F6_evoked rdf:type owl:ObjectProperty ;
             rdfs:subPropertyOf crm:P15_was_influenced_by ;
             rdfs:domain od:L3_Sensory_Experience ;
             rdfs:comment "This property associates an instance of L3 Sensory Experience with a (material or conceptual) entity which is evoked during the experience itself. This includes memories of people or situations, comparison to similar stimuli, references, etc."@en .


###  http://data.odeuropa.eu/ontology/F7_has_species
od:F7_has_species rdf:type owl:ObjectProperty ;
                  rdfs:subPropertyOf crm:P137_exemplifies ;
                  rdf:type owl:AsymmetricProperty ;
                  rdfs:domain od:L6_Animal ;
                  rdfs:range crm:E55_Type ;
                  rdfs:comment "This property associates an instance of L6 Animal with its species, e.g. dog, cat, horse, etc."@en ;
                  owl:cardinality "1"^^xsd:nonNegativeInteger .


###  http://data.odeuropa.eu/ontology/F8_has_nose_quality
od:F8_has_nose_quality rdf:type owl:ObjectProperty ;
                       rdfs:domain crm:E39_Actor ;
                       rdfs:range crm:E55_Type ;
                       rdfs:comment """This property associates an instance of E39 Actor with a quality about their olfaction.

Examples:
* Subtle
* Delicate
* Good"""@en .


###  http://data.odeuropa.eu/ontology/F9_involved_smell
od:F9_involved_smell rdf:type owl:ObjectProperty ;
                     rdfs:domain od:L16_Odorizing ;
                     rdfs:range od:L11_Smell ;
                     rdfs:comment "This property associates an instance of L16 Odorizing with the L11 Smell which has be used for the intended purpose."@en .


#################################################################
#    Classes
#################################################################

###  http://data.odeuropa.eu/ontology/L11_Smell
od:L11_Smell rdf:type owl:Class ;
             rdfs:subClassOf od:L1_Sensory_Stimulus ;
             rdfs:comment """This class comprises all olfactory stimuli, or smells, considered as unique and un-repeatable, possibly existing in a specific time and place, to not be confused with possible generalisation.

Example:
* The smell of a specific rose in my garden in a rainy day (and not the general smell of roses)"""@en .


###  http://data.odeuropa.eu/ontology/L12_Smell_Emission
od:L12_Smell_Emission rdf:type owl:Class ;
                      rdfs:subClassOf od:L2_Stimulus_Generation ;
                      rdfs:comment """This class comprises events in which a specific smell has been generated, either by human intervention or because of natural phenomena.

Examples:
* The eruption of Vesuvius in 79 d.C. emitted sulphuric smells (Pliny the Younger, Epistulae)
* A perfumed candle is emitting good smell of lavender"""@en .


###  http://data.odeuropa.eu/ontology/L13_Olfactory_Experience
od:L13_Olfactory_Experience rdf:type owl:Class ;
                            rdfs:subClassOf od:L3_Sensory_Experience ;
                            rdfs:comment "This class comprises activities in which an actor (human or animal) is perceiving a smell"@en .


###  http://data.odeuropa.eu/ontology/L14_Smell_Transformation
od:L14_Smell_Transformation rdf:type owl:Class ;
                            rdfs:subClassOf od:L4_Stimuli_Transformation ;
                            rdfs:comment """This class comprises events in which a specific smell is transformed into a new one, which somehow differs from the original.

Examples:
* The smells of the fied fish is reduced in intensity by opening the window of the kitchen."""@en .


###  http://data.odeuropa.eu/ontology/L15_Smell_Interaction
od:L15_Smell_Interaction rdf:type owl:Class ;
                         rdfs:subClassOf od:L14_Smell_Transformation ,
                                         od:L5_Stimuli_Interaction ;
                         rdfs:comment """This class comprises events in which two or more specific sensory stimuli interact and create a new combined stimulus, either by human intervention or because of natural phenomena. The different original stimuli are still distinctly existing.

Examples:
* By playing together, the sounds of each instrument of the orchestra are merged in the symphony
* The smells coming from several dishes are combined in the smell of the kitchen environment"""@en .


###  http://data.odeuropa.eu/ontology/L16_Odorizing
od:L16_Odorizing rdf:type owl:Class ;
                 rdfs:subClassOf crm:E7_Activity ;
                 rdfs:comment """This class comprises actions involving intentionally using an odour for a specific purpose.

Example:
* A woman is putting perfume on her body as hygienic practice
* A perfuming substance is used to cover bad smells in the house
* A person likes to smell lavender because this makes her happy"""@en .


###  http://data.odeuropa.eu/ontology/L1_Sensory_Stimulus
od:L1_Sensory_Stimulus rdf:type owl:Class ;
                       rdfs:subClassOf crm:E18_Physical_Thing ,
                                       crmsci:S15_Observable_Entity ;
                       rdfs:comment """This class comprises all kind of stimuli which can be perceived by senses, such as a specific image, smell, taste, sound, etc.
The stimulus described by this class is unique and un-repeatable, possibly existing in a specific time and place, to not be confused with possible generalisation.

Example:
* The smell of a specific rose in my garden in a rainy day (and not the general smell of roses)
* The sound of the bells of Notre Dame de Nice
* The taste of the ice cream I have eaten in Palermo when I was a kid"""@en .


###  http://data.odeuropa.eu/ontology/L2_Stimulus_Generation
od:L2_Stimulus_Generation rdf:type owl:Class ;
                          rdfs:subClassOf crm:E63_Beginning_of_Existence ;
                          rdfs:comment """This class comprises events in which a specific sensory stimulus has been generated, either by human intervention or because of natural phenomena.

Examples:
* The violin playing produces a sound
* The eruption of Vesuvius in 79 d.C. emitted sulphuric smells (Pliny the Younger, Epistulae)"""@en .


###  http://data.odeuropa.eu/ontology/L3_Sensory_Experience
od:L3_Sensory_Experience rdf:type owl:Class ;
                         rdfs:subClassOf crmsci:S4_Observation ;
                         rdfs:comment "This class comprises activities in which an actor (human or animal) is perceiving a stimulus, namely any action of viewing, smelling, listening, tasting, touching."@en .


###  http://data.odeuropa.eu/ontology/L4_Stimuli_Transformation
od:L4_Stimuli_Transformation rdf:type owl:Class ;
                             rdfs:subClassOf crm:E81_Transformation ;
                             rdfs:comment """This class comprises events in which a specific sensory stimuli is transformed into a new one, which somehow differs from the original.

Examples:
* The sound of the organ arrives to the perceived transformed by the echo of the church
* The smells of the fied fish is reduced in intensity by opening the window of the kitchen."""@en .


###  http://data.odeuropa.eu/ontology/L5_Stimuli_Interaction
od:L5_Stimuli_Interaction rdf:type owl:Class ;
                          rdfs:subClassOf od:L4_Stimuli_Transformation ;
                          rdfs:comment """This class comprises events in which two or more specific sensory stimuli interact and create a new combined stimulus, either by human intervention or because of natural phenomena. The different original stimuli are still distinctly existing.

Examples:
* By playing together, the sounds of each instrument of the orchestra are merged in the symphony
* The smells coming from several dishes are combined in the smell of the kitchen environment"""@en .


###  http://data.odeuropa.eu/ontology/L6_Animal
od:L6_Animal rdf:type owl:Class ;
             rdfs:subClassOf crm:E39_Actor ;
             rdfs:comment "This class comprises animals who live or are assumed to have lived. A person is not falling in this class, but rather in E21 Person."@en .


###  http://data.odeuropa.eu/ontology/L7_Gesture
od:L7_Gesture rdf:type owl:Class ;
              rdfs:subClassOf crm:E7_Activity ;
              rdfs:comment """This class comprises actions which are made of a single gesture.

Example:
* Yawning
* Covering the nose"""@en .
