<?xml version="1.0"?>
<rdf:RDF xmlns="http://www.meteck.org/files/ontologies/stuff.owl#"
     xml:base="http://www.meteck.org/files/ontologies/stuff.owl"
     xmlns:rdf="http://www.w3.org/1999/02/22-rdf-syntax-ns#"
     xmlns:owl="http://www.w3.org/2002/07/owl#"
     xmlns:xml="http://www.w3.org/XML/1998/namespace"
     xmlns:om-1="http://www.wurvoc.org/vocabularies/om-1.8/"
     xmlns:xsd="http://www.w3.org/2001/XMLSchema#"
     xmlns:skos="http://www.w3.org/2004/02/skos/core#"
     xmlns:bibo="http://purl.org/ontology/bibo/"
     xmlns:rdfs="http://www.w3.org/2000/01/rdf-schema#"
     xmlns:foaf="http://xmlns.com/foaf/0.1/"
     xmlns:dc="http://purl.org/dc/elements/1.1/"
     xmlns:WV="http://www.wurvoc.org/vocabularies/WV/">
    <owl:Ontology rdf:about="http://www.meteck.org/files/ontologies/stuff.owl">
        <owl:imports rdf:resource="http://www.meteck.org/files/ontologies/OMmini.owl"/>
        <rdfs:comment xml:lang="en">This is the second version of an ontology about stuffkinds (v1.0, d.d. 11-04-2012, v1.5, d.d. 25-6-2014), developed by C. Maria Keet. The paper that describes the details: 
Keet, C.M. A core ontology of macroscopic stuff. 19th International Conference on Knowledge Engineering and Knowledge Management (EKAW&apos;14). K. Janowicz et al. (Eds.). 24-28 Nov, 2014, Linkoping, Sweden. Springer LNAI vol. 8876, 209-224
For questions and comments, please write an email to mkeet@cs.uct.ac.za.</rdfs:comment>
        <rdfs:comment xml:lang="en">This is the third version of the stuff ontology (July 2016). The main updates are the stuff relations (portions and stuff-parts/ingredients) and the import of a module of the OM ontology.</rdfs:comment>
    </owl:Ontology>
    


    <!-- 
    ///////////////////////////////////////////////////////////////////////////////////////
    //
    // Annotation properties
    //
    ///////////////////////////////////////////////////////////////////////////////////////
     -->

    


    <!-- http://www.w3.org/2002/07/owl#qualifiedCardinality -->

    <owl:AnnotationProperty rdf:about="http://www.w3.org/2002/07/owl#qualifiedCardinality"/>
    


    <!-- 
    ///////////////////////////////////////////////////////////////////////////////////////
    //
    // Object Properties
    //
    ///////////////////////////////////////////////////////////////////////////////////////
     -->

    


    <!-- http://www.meteck.org/files/ontologies/stuff.owl#colloidFormingRelation -->

    <owl:ObjectProperty rdf:about="http://www.meteck.org/files/ontologies/stuff.owl#colloidFormingRelation">
        <rdfs:subPropertyOf rdf:resource="http://www.meteck.org/files/ontologies/stuff.owl#stuffFormingRelation"/>
        <rdfs:domain rdf:resource="http://www.meteck.org/files/ontologies/stuff.owl#ContinuousMedium"/>
        <rdfs:range rdf:resource="http://www.meteck.org/files/ontologies/stuff.owl#DispersedPhase"/>
        <rdfs:comment>this one is for the colloids, which also takes care of the surface tension etc. (and does not necessarily involve a chemical reaction like with the solutions)</rdfs:comment>
    </owl:ObjectProperty>
    


    <!-- http://www.meteck.org/files/ontologies/stuff.owl#containedIn -->

    <owl:ObjectProperty rdf:about="http://www.meteck.org/files/ontologies/stuff.owl#containedIn">
        <rdfs:subPropertyOf rdf:resource="http://www.meteck.org/files/ontologies/stuff.owl#partOf"/>
    </owl:ObjectProperty>
    


    <!-- http://www.meteck.org/files/ontologies/stuff.owl#contiguousPortion -->

    <owl:ObjectProperty rdf:about="http://www.meteck.org/files/ontologies/stuff.owl#contiguousPortion">
        <rdfs:subPropertyOf rdf:resource="http://www.meteck.org/files/ontologies/stuff.owl#hasProperPart"/>
        <owl:inverseOf rdf:resource="http://www.meteck.org/files/ontologies/stuff.owl#isContiguousPortionOf"/>
    </owl:ObjectProperty>
    


    <!-- http://www.meteck.org/files/ontologies/stuff.owl#hasContainedScatteredPortion -->

    <owl:ObjectProperty rdf:about="http://www.meteck.org/files/ontologies/stuff.owl#hasContainedScatteredPortion">
        <rdfs:subPropertyOf rdf:resource="http://www.meteck.org/files/ontologies/stuff.owl#scatterPortion"/>
        <owl:inverseOf rdf:resource="http://www.meteck.org/files/ontologies/stuff.owl#isContainedScatteredPortionOf"/>
        <rdfs:comment xml:lang="en">these scattered portions are necessarily contained in a container (such as a glass)</rdfs:comment>
    </owl:ObjectProperty>
    


    <!-- http://www.meteck.org/files/ontologies/stuff.owl#hasGranuleType -->

    <owl:ObjectProperty rdf:about="http://www.meteck.org/files/ontologies/stuff.owl#hasGranuleType">
        <rdfs:subPropertyOf rdf:resource="http://www.w3.org/2002/07/owl#topObjectProperty"/>
        <rdfs:domain rdf:resource="http://www.meteck.org/files/ontologies/stuff.owl#Stuff"/>
        <rdfs:range rdf:resource="http://www.meteck.org/files/ontologies/stuff.owl#PhysicalObject"/>
        <rdfs:comment>terms like &apos;has grain&apos; and &apos;has granular part&apos; tend to be used for this relation as well. but lots of stuffs use bases that are not of one single type/grain/level of granularity (i.e., not only atoms or only molecules or only multi-molecular object). What one does do, is define the basis for analysis, with an implict &apos;we don&apos;t look any more fine-grained than that, and this is out level of analysis&apos;, like, say, the H2O molecules water is composed of, not the p-orbitals or neutrons of those water molecules.
then there&apos;s one thing with asserting &apos;we go as far as the molecules, not below&apos; for some kind/category of stuff and another one to assert that SugaryWater is composed of (or has component) water and sugar, which is asserting the composition at the molecule level and as macroscopic stuffs, and based on that analysis at that level, it is a solution.</rdfs:comment>
    </owl:ObjectProperty>
    


    <!-- http://www.meteck.org/files/ontologies/stuff.owl#hasPart -->

    <owl:ObjectProperty rdf:about="http://www.meteck.org/files/ontologies/stuff.owl#hasPart">
        <owl:inverseOf rdf:resource="http://www.meteck.org/files/ontologies/stuff.owl#partOf"/>
        <rdfs:comment xml:lang="en">concerning some possible hasComponent and composedOf sub-property for stuffs: is hasComponent == composedOf? Somehow, the composedOf seem &apos;essential&apos;, whereas an hasComponent less so, but I can&apos;t nail it down. vodka has component alcohol, but it is not composed of alcohol. One is an object-centred view with a &apos;z happens to have x and y as components&apos;, the other a process-centred view with an &apos;we put x and y together to obtain z&apos;. Example: wine happens to have alcohol thanks to the fermentation, but for whipped cream, we put air and cream together. This deserves closer scrutiny, but is an orthogonal aspect.</rdfs:comment>
        <rdfs:comment xml:lang="en">note: domain and range axioms, where applicable, are declared in the part-of branch (the inverses) only (as it infers them here then).</rdfs:comment>
    </owl:ObjectProperty>
    


    <!-- http://www.meteck.org/files/ontologies/stuff.owl#hasPartStuff -->

    <owl:ObjectProperty rdf:about="http://www.meteck.org/files/ontologies/stuff.owl#hasPartStuff">
        <rdfs:subPropertyOf rdf:resource="http://www.meteck.org/files/ontologies/stuff.owl#hasProperPart"/>
        <owl:inverseOf rdf:resource="http://www.meteck.org/files/ontologies/stuff.owl#stuffPartOf"/>
        <rdfs:comment xml:lang="en">What the domain and range axiom fail to capture is that they have to be distinct kinds of stuffs.</rdfs:comment>
    </owl:ObjectProperty>
    


    <!-- http://www.meteck.org/files/ontologies/stuff.owl#hasPortion -->

    <owl:ObjectProperty rdf:about="http://www.meteck.org/files/ontologies/stuff.owl#hasPortion">
        <rdfs:subPropertyOf rdf:resource="http://www.meteck.org/files/ontologies/stuff.owl#hasProperPart"/>
        <owl:inverseOf rdf:resource="http://www.meteck.org/files/ontologies/stuff.owl#portionOf"/>
        <rdfs:comment xml:lang="en">Note that, when any of the portions, or portions of the portions, loses some molecules due to some reaction or radioactive degradation (not due to phase change), then the original quantity ceases to exist. according to philosphers. Given that that happens pretty much continuously, then in the strict sense, there isn&apos;t much point in talking of portions. Practically, they are useful though (&apos;naive chemistry&apos;, if you will)</rdfs:comment>
        <rdfs:comment xml:lang="en">a part that is of the same stuffkind as its whole. (not reflected as such in the OWL ontology, due to expressiveness limtations)
Example: the top-half of the wine in my glass and the bottom-half are portions of the whole amount of wine in my wine glass (assume this is instantaneous division [recolelction motin of molecules]), the wine in the wineglass was/is a portion of the amount that was in the wine bottle, etc.
</rdfs:comment>
    </owl:ObjectProperty>
    


    <!-- http://www.meteck.org/files/ontologies/stuff.owl#hasProperPart -->

    <owl:ObjectProperty rdf:about="http://www.meteck.org/files/ontologies/stuff.owl#hasProperPart">
        <rdfs:subPropertyOf rdf:resource="http://www.meteck.org/files/ontologies/stuff.owl#hasPart"/>
        <owl:inverseOf rdf:resource="http://www.meteck.org/files/ontologies/stuff.owl#properPartOf"/>
    </owl:ObjectProperty>
    


    <!-- http://www.meteck.org/files/ontologies/stuff.owl#hasQuale -->

    <owl:ObjectProperty rdf:about="http://www.meteck.org/files/ontologies/stuff.owl#hasQuale">
        <rdfs:domain rdf:resource="http://www.meteck.org/files/ontologies/stuff.owl#Quality"/>
        <rdfs:range rdf:resource="http://www.meteck.org/files/ontologies/stuff.owl#Abstract"/>
    </owl:ObjectProperty>
    


    <!-- http://www.meteck.org/files/ontologies/stuff.owl#hasQuality -->

    <owl:ObjectProperty rdf:about="http://www.meteck.org/files/ontologies/stuff.owl#hasQuality">
        <rdfs:domain>
            <owl:Class>
                <owl:unionOf rdf:parseType="Collection">
                    <rdf:Description rdf:about="http://www.meteck.org/files/ontologies/stuff.owl#Endurant"/>
                    <rdf:Description rdf:about="http://www.meteck.org/files/ontologies/stuff.owl#Perdurant"/>
                </owl:unionOf>
            </owl:Class>
        </rdfs:domain>
        <rdfs:range rdf:resource="http://www.meteck.org/files/ontologies/stuff.owl#Quality"/>
    </owl:ObjectProperty>
    


    <!-- http://www.meteck.org/files/ontologies/stuff.owl#hasScatterStuffPart -->

    <owl:ObjectProperty rdf:about="http://www.meteck.org/files/ontologies/stuff.owl#hasScatterStuffPart">
        <rdfs:subPropertyOf rdf:resource="http://www.meteck.org/files/ontologies/stuff.owl#hasProperPart"/>
        <owl:inverseOf rdf:resource="http://www.meteck.org/files/ontologies/stuff.owl#scatteredStuffPartOf"/>
    </owl:ObjectProperty>
    


    <!-- http://www.meteck.org/files/ontologies/stuff.owl#hasSelfContainedScatteredPortion -->

    <owl:ObjectProperty rdf:about="http://www.meteck.org/files/ontologies/stuff.owl#hasSelfContainedScatteredPortion">
        <rdfs:subPropertyOf rdf:resource="http://www.meteck.org/files/ontologies/stuff.owl#scatterPortion"/>
        <owl:inverseOf rdf:resource="http://www.meteck.org/files/ontologies/stuff.owl#isSelfContainedScatteredPortionOf"/>
        <rdfs:comment xml:lang="en">this if for the pieces, such as lumps, puddle, slice, etc.</rdfs:comment>
    </owl:ObjectProperty>
    


    <!-- http://www.meteck.org/files/ontologies/stuff.owl#hasState -->

    <owl:ObjectProperty rdf:about="http://www.meteck.org/files/ontologies/stuff.owl#hasState">
        <rdfs:subPropertyOf rdf:resource="http://www.w3.org/2002/07/owl#topObjectProperty"/>
        <rdfs:domain rdf:resource="http://www.meteck.org/files/ontologies/stuff.owl#PhysicalEndurant"/>
        <rdfs:range rdf:resource="http://www.meteck.org/files/ontologies/stuff.owl#State"/>
    </owl:ObjectProperty>
    


    <!-- http://www.meteck.org/files/ontologies/stuff.owl#hasStuffDistribution -->

    <owl:ObjectProperty rdf:about="http://www.meteck.org/files/ontologies/stuff.owl#hasStuffDistribution"/>
    


    <!-- http://www.meteck.org/files/ontologies/stuff.owl#inheresIn -->

    <owl:ObjectProperty rdf:about="http://www.meteck.org/files/ontologies/stuff.owl#inheresIn">
        <rdfs:domain rdf:resource="http://www.meteck.org/files/ontologies/stuff.owl#Role"/>
        <rdfs:range rdf:resource="http://www.meteck.org/files/ontologies/stuff.owl#PhysicalEndurant"/>
    </owl:ObjectProperty>
    


    <!-- http://www.meteck.org/files/ontologies/stuff.owl#instantiation -->

    <owl:ObjectProperty rdf:about="http://www.meteck.org/files/ontologies/stuff.owl#instantiation">
        <rdfs:domain rdf:resource="http://www.meteck.org/files/ontologies/stuff.owl#AmountOfStuff"/>
        <rdfs:range rdf:resource="http://www.meteck.org/files/ontologies/stuff.owl#Stuff"/>
        <rdfs:comment xml:lang="en">this object property is intentionally typed, so as to not use it elsewhere than for this case of putting 1st and 2nd order in the same ontology in the TBox. Particular amounts of matter are instances of some type of stuff, like 1kg of gold is an instance of the stuff Gold.</rdfs:comment>
    </owl:ObjectProperty>
    


    <!-- http://www.meteck.org/files/ontologies/stuff.owl#isContainedScatteredPortionOf -->

    <owl:ObjectProperty rdf:about="http://www.meteck.org/files/ontologies/stuff.owl#isContainedScatteredPortionOf">
        <rdfs:subPropertyOf rdf:resource="http://www.meteck.org/files/ontologies/stuff.owl#scatteredPortionOf"/>
        <rdfs:domain>
            <owl:Class>
                <owl:unionOf rdf:parseType="Collection">
                    <rdf:Description rdf:about="http://www.meteck.org/files/ontologies/stuff.owl#AmountOfStuff"/>
                    <rdf:Description rdf:about="http://www.meteck.org/files/ontologies/stuff.owl#Stuff"/>
                </owl:unionOf>
            </owl:Class>
        </rdfs:domain>
        <rdfs:range>
            <owl:Class>
                <owl:unionOf rdf:parseType="Collection">
                    <rdf:Description rdf:about="http://www.meteck.org/files/ontologies/stuff.owl#AmountOfStuff"/>
                    <rdf:Description rdf:about="http://www.meteck.org/files/ontologies/stuff.owl#Stuff"/>
                </owl:unionOf>
            </owl:Class>
        </rdfs:range>
        <rdfs:comment xml:lang="en">this portion *was* a portion of a larger amount of stuff; it needs a container. (cf. self-contained portion)
example: the wine in the wine glass is a scattered portion of the total amount that was in the wine bottle</rdfs:comment>
    </owl:ObjectProperty>
    


    <!-- http://www.meteck.org/files/ontologies/stuff.owl#isContiguousPortionOf -->

    <owl:ObjectProperty rdf:about="http://www.meteck.org/files/ontologies/stuff.owl#isContiguousPortionOf">
        <rdfs:subPropertyOf rdf:resource="http://www.meteck.org/files/ontologies/stuff.owl#properPartOf"/>
        <rdfs:domain>
            <owl:Class>
                <owl:unionOf rdf:parseType="Collection">
                    <rdf:Description rdf:about="http://www.meteck.org/files/ontologies/stuff.owl#AmountOfStuff"/>
                    <rdf:Description rdf:about="http://www.meteck.org/files/ontologies/stuff.owl#Stuff"/>
                </owl:unionOf>
            </owl:Class>
        </rdfs:domain>
        <rdfs:range>
            <owl:Class>
                <owl:unionOf rdf:parseType="Collection">
                    <rdf:Description rdf:about="http://www.meteck.org/files/ontologies/stuff.owl#AmountOfStuff"/>
                    <rdf:Description rdf:about="http://www.meteck.org/files/ontologies/stuff.owl#Stuff"/>
                </owl:unionOf>
            </owl:Class>
        </rdfs:range>
        <rdfs:comment xml:lang="en">This property is supposed to be a suproperty of portionOf, but then the chains involving portionOf would be prohibited (it leads to a cycle, and those cycles lead to undecidability). Because DL reasoners do not do much with the hierarchy in the RBox and the semantic differences between these properties---temporality---cannot be represented in OWL anyway, they are made siblings, for the inferences with the property chains are deemed more important.</rdfs:comment>
    </owl:ObjectProperty>
    


    <!-- http://www.meteck.org/files/ontologies/stuff.owl#isSelfContainedScatteredPortionOf -->

    <owl:ObjectProperty rdf:about="http://www.meteck.org/files/ontologies/stuff.owl#isSelfContainedScatteredPortionOf">
        <rdfs:subPropertyOf rdf:resource="http://www.meteck.org/files/ontologies/stuff.owl#scatteredPortionOf"/>
        <rdfs:domain>
            <owl:Class>
                <owl:unionOf rdf:parseType="Collection">
                    <rdf:Description rdf:about="http://www.meteck.org/files/ontologies/stuff.owl#AmountOfStuff"/>
                    <rdf:Description rdf:about="http://www.meteck.org/files/ontologies/stuff.owl#Stuff"/>
                </owl:unionOf>
            </owl:Class>
        </rdfs:domain>
        <rdfs:range>
            <owl:Class>
                <owl:unionOf rdf:parseType="Collection">
                    <rdf:Description rdf:about="http://www.meteck.org/files/ontologies/stuff.owl#AmountOfStuff"/>
                    <rdf:Description rdf:about="http://www.meteck.org/files/ontologies/stuff.owl#Stuff"/>
                </owl:unionOf>
            </owl:Class>
        </rdfs:range>
        <rdfs:comment xml:lang="en">this portion *was* a portion of a larger amount of stuff; it is a self-standing piece (e.g., a lump, drop, slide). (cf. contiguous portion)
example: the slice of the cake was part of the cake</rdfs:comment>
    </owl:ObjectProperty>
    


    <!-- http://www.meteck.org/files/ontologies/stuff.owl#partOf -->

    <owl:ObjectProperty rdf:about="http://www.meteck.org/files/ontologies/stuff.owl#partOf">
        <rdf:type rdf:resource="http://www.w3.org/2002/07/owl#TransitiveProperty"/>
    </owl:ObjectProperty>
    


    <!-- http://www.meteck.org/files/ontologies/stuff.owl#portionOf -->

    <owl:ObjectProperty rdf:about="http://www.meteck.org/files/ontologies/stuff.owl#portionOf">
        <rdfs:subPropertyOf rdf:resource="http://www.meteck.org/files/ontologies/stuff.owl#properPartOf"/>
        <rdfs:domain>
            <owl:Class>
                <owl:unionOf rdf:parseType="Collection">
                    <rdf:Description rdf:about="http://www.meteck.org/files/ontologies/stuff.owl#AmountOfStuff"/>
                    <rdf:Description rdf:about="http://www.meteck.org/files/ontologies/stuff.owl#Stuff"/>
                </owl:unionOf>
            </owl:Class>
        </rdfs:domain>
        <rdfs:range>
            <owl:Class>
                <owl:unionOf rdf:parseType="Collection">
                    <rdf:Description rdf:about="http://www.meteck.org/files/ontologies/stuff.owl#AmountOfStuff"/>
                    <rdf:Description rdf:about="http://www.meteck.org/files/ontologies/stuff.owl#Stuff"/>
                </owl:unionOf>
            </owl:Class>
        </rdfs:range>
        <rdfs:comment>relation between amounts of matter or stuffs (like gold, milk, mayonnaise), i.e., those entities that are in natural langauge indicated with mass nouns and are not countable, or only countable in amounts of the stuff.
this one is specific for a stuff and a portion that is of the *same* type of stuff. (cf. stuff-part)
examples: slice of the cake is a portion of the cake, glass of wine is a portion of the bottle of wine, etc.</rdfs:comment>
    </owl:ObjectProperty>
    


    <!-- http://www.meteck.org/files/ontologies/stuff.owl#properContainedIn -->

    <owl:ObjectProperty rdf:about="http://www.meteck.org/files/ontologies/stuff.owl#properContainedIn">
        <rdfs:subPropertyOf rdf:resource="http://www.meteck.org/files/ontologies/stuff.owl#properPartOf"/>
    </owl:ObjectProperty>
    


    <!-- http://www.meteck.org/files/ontologies/stuff.owl#properPartOf -->

    <owl:ObjectProperty rdf:about="http://www.meteck.org/files/ontologies/stuff.owl#properPartOf">
        <rdfs:subPropertyOf rdf:resource="http://www.meteck.org/files/ontologies/stuff.owl#partOf"/>
        <rdfs:comment xml:lang="en">usual proper parthood in mereology</rdfs:comment>
    </owl:ObjectProperty>
    


    <!-- http://www.meteck.org/files/ontologies/stuff.owl#scatterPortion -->

    <owl:ObjectProperty rdf:about="http://www.meteck.org/files/ontologies/stuff.owl#scatterPortion">
        <rdfs:subPropertyOf rdf:resource="http://www.meteck.org/files/ontologies/stuff.owl#hasProperPart"/>
        <owl:inverseOf rdf:resource="http://www.meteck.org/files/ontologies/stuff.owl#scatteredPortionOf"/>
        <rdfs:comment xml:lang="en">like portion, but then the temporal aspect to it: some portion x of y was a  contiguous part of y at time t and that portion x is now on the moon at time t&apos; (with t&apos;&gt;t). Mundane example: the wine in the wine glass you just poured from the wine in the wine bottle, the slice of bread that you just sliced from the loaf of bread.
For the modelling, it might perhaps be useful to have two subproperties: one for  (sub)portions that each come with its container, and one that does not. It&apos;s one thing to talk of lumps, puddles, slices etc. that merely give a vague indication of the amount and are &apos;selfstanding&apos; amounts, and another that needs to have the container recorded with it, like a silo of grain, cup of tea, sachet of sugar. </rdfs:comment>
    </owl:ObjectProperty>
    


    <!-- http://www.meteck.org/files/ontologies/stuff.owl#scatteredPortionOf -->

    <owl:ObjectProperty rdf:about="http://www.meteck.org/files/ontologies/stuff.owl#scatteredPortionOf">
        <rdfs:subPropertyOf rdf:resource="http://www.meteck.org/files/ontologies/stuff.owl#properPartOf"/>
        <rdfs:domain>
            <owl:Class>
                <owl:unionOf rdf:parseType="Collection">
                    <rdf:Description rdf:about="http://www.meteck.org/files/ontologies/stuff.owl#AmountOfStuff"/>
                    <rdf:Description rdf:about="http://www.meteck.org/files/ontologies/stuff.owl#Stuff"/>
                </owl:unionOf>
            </owl:Class>
        </rdfs:domain>
        <rdfs:range>
            <owl:Class>
                <owl:unionOf rdf:parseType="Collection">
                    <rdf:Description rdf:about="http://www.meteck.org/files/ontologies/stuff.owl#AmountOfStuff"/>
                    <rdf:Description rdf:about="http://www.meteck.org/files/ontologies/stuff.owl#Stuff"/>
                </owl:unionOf>
            </owl:Class>
        </rdfs:range>
        <owl:propertyChainAxiom rdf:parseType="Collection">
            <rdf:Description rdf:about="http://www.meteck.org/files/ontologies/stuff.owl#scatteredPortionOf"/>
            <rdf:Description rdf:about="http://www.meteck.org/files/ontologies/stuff.owl#portionOf"/>
        </owl:propertyChainAxiom>
        <rdfs:comment xml:lang="en">This property is supposed to be a suproperty of portionOf, but then the chain &quot;scatteredPortionOf o portionOf isa scatteredPortionOf&quot; is prohibited (it leads to a cycle, because scatteredPortionOf \isa portion, and those cycles lead to undecidability). Because DL reasoners do not do much with the hierarchy in the RBox and the semantic differences between these properties---temporality---cannot be represented in OWL anyway, they are made siblings, for the inferences with the property chains are deemed more important.</rdfs:comment>
    </owl:ObjectProperty>
    


    <!-- http://www.meteck.org/files/ontologies/stuff.owl#scatteredStuffPartOf -->

    <owl:ObjectProperty rdf:about="http://www.meteck.org/files/ontologies/stuff.owl#scatteredStuffPartOf">
        <rdfs:subPropertyOf rdf:resource="http://www.meteck.org/files/ontologies/stuff.owl#properPartOf"/>
        <rdfs:domain>
            <owl:Class>
                <owl:unionOf rdf:parseType="Collection">
                    <rdf:Description rdf:about="http://www.meteck.org/files/ontologies/stuff.owl#AmountOfStuff"/>
                    <rdf:Description rdf:about="http://www.meteck.org/files/ontologies/stuff.owl#Stuff"/>
                </owl:unionOf>
            </owl:Class>
        </rdfs:domain>
        <rdfs:range>
            <owl:Class>
                <owl:unionOf rdf:parseType="Collection">
                    <rdf:Description rdf:about="http://www.meteck.org/files/ontologies/stuff.owl#AmountOfStuff"/>
                    <rdf:Description rdf:about="http://www.meteck.org/files/ontologies/stuff.owl#Stuff"/>
                </owl:unionOf>
            </owl:Class>
        </rdfs:range>
        <owl:propertyChainAxiom rdf:parseType="Collection">
            <rdf:Description rdf:about="http://www.meteck.org/files/ontologies/stuff.owl#stuffPartOf"/>
            <rdf:Description rdf:about="http://www.meteck.org/files/ontologies/stuff.owl#contiguousPortion"/>
            <rdf:Description rdf:about="http://www.meteck.org/files/ontologies/stuff.owl#isSelfContainedScatteredPortionOf"/>
        </owl:propertyChainAxiom>
        <rdfs:comment xml:lang="en">this is supposed to be a subproperty of stuffpartOf, relating  amounts of matter or stuffs (like gold, milk, mayonnaise), i.e., those entities that are in natural language indicated with mass nouns and are not countable, or only countable in amounts of the stuff. This one is specific for a stuff and its &apos;ingredient&apos; that is of *another* type of stuff. (cf. portions). examples: alcohol is a stuff-part of wine, oil in mayonnaise, sugar in cake etc.

but then the property chains won&apos;t work, due to cycles.

And it is supposed to be a termporalised relation, in that the scattereed part *was* a contiguous proper part of the whole.</rdfs:comment>
    </owl:ObjectProperty>
    


    <!-- http://www.meteck.org/files/ontologies/stuff.owl#solutionFormingRelation -->

    <owl:ObjectProperty rdf:about="http://www.meteck.org/files/ontologies/stuff.owl#solutionFormingRelation">
        <rdfs:subPropertyOf rdf:resource="http://www.meteck.org/files/ontologies/stuff.owl#stuffFormingRelation"/>
        <rdfs:domain rdf:resource="http://www.meteck.org/files/ontologies/stuff.owl#Solvent"/>
        <rdfs:range rdf:resource="http://www.meteck.org/files/ontologies/stuff.owl#Solute"/>
        <rdfs:comment>this one is for chemically dissolving one stuff in another</rdfs:comment>
    </owl:ObjectProperty>
    


    <!-- http://www.meteck.org/files/ontologies/stuff.owl#srInheresIn -->

    <owl:ObjectProperty rdf:about="http://www.meteck.org/files/ontologies/stuff.owl#srInheresIn">
        <rdfs:subPropertyOf rdf:resource="http://www.meteck.org/files/ontologies/stuff.owl#inheresIn"/>
        <rdfs:domain rdf:resource="http://www.meteck.org/files/ontologies/stuff.owl#StuffRole"/>
        <rdfs:range rdf:resource="http://www.meteck.org/files/ontologies/stuff.owl#Stuff"/>
    </owl:ObjectProperty>
    


    <!-- http://www.meteck.org/files/ontologies/stuff.owl#stuffFormingRelation -->

    <owl:ObjectProperty rdf:about="http://www.meteck.org/files/ontologies/stuff.owl#stuffFormingRelation">
        <rdfs:domain>
            <owl:Class>
                <owl:unionOf rdf:parseType="Collection">
                    <rdf:Description rdf:about="http://www.meteck.org/files/ontologies/stuff.owl#ContinuousMedium"/>
                    <rdf:Description rdf:about="http://www.meteck.org/files/ontologies/stuff.owl#DispersedPhase"/>
                    <rdf:Description rdf:about="http://www.meteck.org/files/ontologies/stuff.owl#Solute"/>
                    <rdf:Description rdf:about="http://www.meteck.org/files/ontologies/stuff.owl#Solvent"/>
                </owl:unionOf>
            </owl:Class>
        </rdfs:domain>
        <rdfs:range>
            <owl:Class>
                <owl:unionOf rdf:parseType="Collection">
                    <rdf:Description rdf:about="http://www.meteck.org/files/ontologies/stuff.owl#ContinuousMedium"/>
                    <rdf:Description rdf:about="http://www.meteck.org/files/ontologies/stuff.owl#DispersedPhase"/>
                    <rdf:Description rdf:about="http://www.meteck.org/files/ontologies/stuff.owl#Solute"/>
                    <rdf:Description rdf:about="http://www.meteck.org/files/ontologies/stuff.owl#Solvent"/>
                </owl:unionOf>
            </owl:Class>
        </rdfs:range>
        <rdfs:comment>the stuffFormingRelation is now (over?)loaded with the semantics of representing the notions that there is a relation forming between the objects in the stuff, like, surface tension of the particles in the colloid, H-bond, and so on, and the ratio as regards to how things are mixed (e.g., we only have lemonade when we have them in a mixture of  water:sugar:lemonjuice in the ratio of, say, 8:1:1, that is, proportional amounts in ml, grams, whatever). </rdfs:comment>
    </owl:ObjectProperty>
    


    <!-- http://www.meteck.org/files/ontologies/stuff.owl#stuffPartOf -->

    <owl:ObjectProperty rdf:about="http://www.meteck.org/files/ontologies/stuff.owl#stuffPartOf">
        <rdfs:subPropertyOf rdf:resource="http://www.meteck.org/files/ontologies/stuff.owl#properPartOf"/>
        <rdfs:domain>
            <owl:Class>
                <owl:unionOf rdf:parseType="Collection">
                    <rdf:Description rdf:about="http://www.meteck.org/files/ontologies/stuff.owl#AmountOfStuff"/>
                    <rdf:Description rdf:about="http://www.meteck.org/files/ontologies/stuff.owl#Stuff"/>
                </owl:unionOf>
            </owl:Class>
        </rdfs:domain>
        <rdfs:range>
            <owl:Class>
                <owl:unionOf rdf:parseType="Collection">
                    <rdf:Description rdf:about="http://www.meteck.org/files/ontologies/stuff.owl#AmountOfStuff"/>
                    <rdf:Description rdf:about="http://www.meteck.org/files/ontologies/stuff.owl#Stuff"/>
                </owl:unionOf>
            </owl:Class>
        </rdfs:range>
        <rdfs:comment xml:lang="en">relation between amounts of matter or stuffs (like gold, milk, mayonnaise), i.e., those entities that are in natural langauge indicated with mass nouns and are not countable, or only countable in amounts of the stuff.
this one is specific for a stuff and its &apos;ingredient&apos; that is of *another* type of stuff. (cf. portions)
examples: alcohol is a stuff-part of wine, oil in mayonnaise, sugar in cake etc.</rdfs:comment>
    </owl:ObjectProperty>
    


    <!-- 
    ///////////////////////////////////////////////////////////////////////////////////////
    //
    // Data properties
    //
    ///////////////////////////////////////////////////////////////////////////////////////
     -->

    


    <!-- http://www.meteck.org/files/ontologies/stuff.owl#hasDataValue -->

    <owl:DatatypeProperty rdf:about="http://www.meteck.org/files/ontologies/stuff.owl#hasDataValue">
        <rdfs:domain rdf:resource="http://www.meteck.org/files/ontologies/stuff.owl#Abstract"/>
        <rdfs:comment>the range should be &apos;any data type&apos;, but it doesn&apos;t allow that anymore, in the sense that when I specilfy elsewhere in an axiom that it is, say, string, then it gives me an error, though theoretically [conceptually, if you will] it shouldn&apos;t. tried literal, tried anyType (rejected outright) and tried anyURI.
workaround: removed range specification. </rdfs:comment>
    </owl:DatatypeProperty>
    


    <!-- http://www.meteck.org/files/ontologies/stuff.owl#hasNrOfPhase -->

    <owl:DatatypeProperty rdf:about="http://www.meteck.org/files/ontologies/stuff.owl#hasNrOfPhase">
        <rdfs:domain rdf:resource="http://www.meteck.org/files/ontologies/stuff.owl#Stuff"/>
        <rdfs:range rdf:resource="http://www.w3.org/2001/XMLSchema#integer"/>
    </owl:DatatypeProperty>
    


    <!-- 
    ///////////////////////////////////////////////////////////////////////////////////////
    //
    // Classes
    //
    ///////////////////////////////////////////////////////////////////////////////////////
     -->

    


    <!-- http://www.meteck.org/files/ontologies/stuff.owl#Abstract -->

    <owl:Class rdf:about="http://www.meteck.org/files/ontologies/stuff.owl#Abstract"/>
    


    <!-- http://www.meteck.org/files/ontologies/stuff.owl#AbstractRegion -->

    <owl:Class rdf:about="http://www.meteck.org/files/ontologies/stuff.owl#AbstractRegion">
        <rdfs:subClassOf rdf:resource="http://www.meteck.org/files/ontologies/stuff.owl#Region"/>
    </owl:Class>
    


    <!-- http://www.meteck.org/files/ontologies/stuff.owl#AmountOfStuff -->

    <owl:Class rdf:about="http://www.meteck.org/files/ontologies/stuff.owl#AmountOfStuff">
        <rdfs:subClassOf rdf:resource="http://www.meteck.org/files/ontologies/stuff.owl#PhysicalEndurant"/>
        <rdfs:comment xml:lang="en">as in dolce&apos;s amount of matter, for particulars only.</rdfs:comment>
    </owl:Class>
    


    <!-- http://www.meteck.org/files/ontologies/stuff.owl#AssociationalColloid -->

    <owl:Class rdf:about="http://www.meteck.org/files/ontologies/stuff.owl#AssociationalColloid">
        <rdfs:subClassOf rdf:resource="http://www.meteck.org/files/ontologies/stuff.owl#Colloid"/>
        <rdfs:comment>like hydrophibic/hydrophilic.
micellar colloids, like soap.
Optionally, one can add properties like the aggregation number (amount of molecules in the micels), which is normally a range, due to the critical micelle concentration adn so on.</rdfs:comment>
    </owl:Class>
    


    <!-- http://www.meteck.org/files/ontologies/stuff.owl#Atom -->

    <owl:Class rdf:about="http://www.meteck.org/files/ontologies/stuff.owl#Atom">
        <rdfs:subClassOf rdf:resource="http://www.meteck.org/files/ontologies/stuff.owl#PhysicalObject"/>
    </owl:Class>
    


    <!-- http://www.meteck.org/files/ontologies/stuff.owl#Bulk -->

    <owl:Class rdf:about="http://www.meteck.org/files/ontologies/stuff.owl#Bulk">
        <rdfs:subClassOf rdf:resource="http://www.meteck.org/files/ontologies/stuff.owl#Stuff"/>
        <rdfs:subClassOf>
            <owl:Class>
                <owl:intersectionOf rdf:parseType="Collection">
                    <owl:Class>
                        <owl:unionOf rdf:parseType="Collection">
                            <owl:Restriction>
                                <owl:onProperty rdf:resource="http://www.meteck.org/files/ontologies/stuff.owl#hasGranuleType"/>
                                <owl:someValuesFrom>
                                    <owl:Class>
                                        <owl:unionOf rdf:parseType="Collection">
                                            <rdf:Description rdf:about="http://www.meteck.org/files/ontologies/stuff.owl#Molecule"/>
                                            <rdf:Description rdf:about="http://www.meteck.org/files/ontologies/stuff.owl#MultiMoleculeParticle"/>
                                        </owl:unionOf>
                                    </owl:Class>
                                </owl:someValuesFrom>
                            </owl:Restriction>
                            <owl:Restriction>
                                <owl:onProperty rdf:resource="http://www.meteck.org/files/ontologies/stuff.owl#hasPartStuff"/>
                                <owl:someValuesFrom rdf:resource="http://www.meteck.org/files/ontologies/stuff.owl#Stuff"/>
                            </owl:Restriction>
                        </owl:unionOf>
                    </owl:Class>
                    <owl:Class>
                        <owl:unionOf rdf:parseType="Collection">
                            <owl:Restriction>
                                <owl:onProperty rdf:resource="http://www.meteck.org/files/ontologies/stuff.owl#hasGranuleType"/>
                                <owl:allValuesFrom>
                                    <owl:Class>
                                        <owl:unionOf rdf:parseType="Collection">
                                            <rdf:Description rdf:about="http://www.meteck.org/files/ontologies/stuff.owl#Molecule"/>
                                            <rdf:Description rdf:about="http://www.meteck.org/files/ontologies/stuff.owl#MultiMoleculeParticle"/>
                                        </owl:unionOf>
                                    </owl:Class>
                                </owl:allValuesFrom>
                            </owl:Restriction>
                            <owl:Restriction>
                                <owl:onProperty rdf:resource="http://www.meteck.org/files/ontologies/stuff.owl#hasPartStuff"/>
                                <owl:allValuesFrom rdf:resource="http://www.meteck.org/files/ontologies/stuff.owl#Stuff"/>
                            </owl:Restriction>
                        </owl:unionOf>
                    </owl:Class>
                </owl:intersectionOf>
            </owl:Class>
        </rdfs:subClassOf>
        <rdfs:subClassOf>
            <owl:Class>
                <owl:unionOf rdf:parseType="Collection">
                    <rdf:Description rdf:about="http://www.meteck.org/files/ontologies/stuff.owl#MixedStuff"/>
                    <rdf:Description rdf:about="http://www.meteck.org/files/ontologies/stuff.owl#StructuredPureStuff"/>
                </owl:unionOf>
            </owl:Class>
        </rdfs:subClassOf>
        <rdfs:comment xml:lang="en">Bulk goods, like (a silo of) soy beans, coffee, nuts, pet food, tea, whole grains, sugar. This term is typically used in the food industry. Flour and honey are indeed kinds of stuff, but, on the face of it, one can count each nut and cookie. However, the latter are, in that context, meant to go only in amounts, not individual nuts or cookies; e.g., a bag of nuts, a packet of cookies. This is just a matter of scale: the basis type of the latter is the nut or cookie instead of the countable molecule, and it goes in quantities, like a bag of peanuts or packet of cookies. In addition, bulk can come as StructuredPureStuff (sugar), HomogenousMixedStuff (the processed peanut butter with the stabilizer and possibly also sugar, not the ones from the health shop that settle and separate in peanut paste and oil on top), and HeterogenousMixedStuff, like pet food and breakfast cereals. Actually, it can be anything, except UnstructuredPureStuff</rdfs:comment>
    </owl:Class>
    


    <!-- http://www.meteck.org/files/ontologies/stuff.owl#Colloid -->

    <owl:Class rdf:about="http://www.meteck.org/files/ontologies/stuff.owl#Colloid">
        <owl:equivalentClass>
            <owl:Class>
                <owl:intersectionOf rdf:parseType="Collection">
                    <rdf:Description rdf:about="http://www.meteck.org/files/ontologies/stuff.owl#HomogeneousMixture"/>
                    <owl:Restriction>
                        <owl:onProperty rdf:resource="http://www.meteck.org/files/ontologies/stuff.owl#hasPartStuff"/>
                        <owl:qualifiedCardinality rdf:datatype="http://www.w3.org/2001/XMLSchema#nonNegativeInteger">1</owl:qualifiedCardinality>
                        <owl:onClass>
                            <owl:Class>
                                <owl:intersectionOf rdf:parseType="Collection">
                                    <rdf:Description rdf:about="http://www.meteck.org/files/ontologies/stuff.owl#Stuff"/>
                                    <owl:Restriction>
                                        <owl:onProperty rdf:resource="http://www.meteck.org/files/ontologies/stuff.owl#hasState"/>
                                        <owl:someValuesFrom rdf:resource="http://www.meteck.org/files/ontologies/stuff.owl#StuffState"/>
                                    </owl:Restriction>
                                    <owl:Restriction>
                                        <owl:onProperty>
                                            <rdf:Description>
                                                <owl:inverseOf rdf:resource="http://www.meteck.org/files/ontologies/stuff.owl#srInheresIn"/>
                                            </rdf:Description>
                                        </owl:onProperty>
                                        <owl:someValuesFrom rdf:resource="http://www.meteck.org/files/ontologies/stuff.owl#ContinuousMedium"/>
                                    </owl:Restriction>
                                </owl:intersectionOf>
                            </owl:Class>
                        </owl:onClass>
                    </owl:Restriction>
                    <owl:Restriction>
                        <owl:onProperty rdf:resource="http://www.meteck.org/files/ontologies/stuff.owl#hasPartStuff"/>
                        <owl:qualifiedCardinality rdf:datatype="http://www.w3.org/2001/XMLSchema#nonNegativeInteger">1</owl:qualifiedCardinality>
                        <owl:onClass>
                            <owl:Class>
                                <owl:intersectionOf rdf:parseType="Collection">
                                    <rdf:Description rdf:about="http://www.meteck.org/files/ontologies/stuff.owl#Stuff"/>
                                    <owl:Restriction>
                                        <owl:onProperty rdf:resource="http://www.meteck.org/files/ontologies/stuff.owl#hasState"/>
                                        <owl:someValuesFrom rdf:resource="http://www.meteck.org/files/ontologies/stuff.owl#StuffState"/>
                                    </owl:Restriction>
                                    <owl:Restriction>
                                        <owl:onProperty>
                                            <rdf:Description>
                                                <owl:inverseOf rdf:resource="http://www.meteck.org/files/ontologies/stuff.owl#srInheresIn"/>
                                            </rdf:Description>
                                        </owl:onProperty>
                                        <owl:someValuesFrom rdf:resource="http://www.meteck.org/files/ontologies/stuff.owl#DispersedPhase"/>
                                    </owl:Restriction>
                                </owl:intersectionOf>
                            </owl:Class>
                        </owl:onClass>
                    </owl:Restriction>
                    <owl:Restriction>
                        <owl:onProperty rdf:resource="http://www.meteck.org/files/ontologies/stuff.owl#hasNrOfPhase"/>
                        <owl:someValuesFrom>
                            <rdfs:Datatype>
                                <owl:onDatatype rdf:resource="http://www.w3.org/2001/XMLSchema#int"/>
                                <owl:withRestrictions rdf:parseType="Collection">
                                    <rdf:Description>
                                        <xsd:minInclusive rdf:datatype="http://www.w3.org/2001/XMLSchema#integer">2</xsd:minInclusive>
                                    </rdf:Description>
                                </owl:withRestrictions>
                            </rdfs:Datatype>
                        </owl:someValuesFrom>
                    </owl:Restriction>
                </owl:intersectionOf>
            </owl:Class>
        </owl:equivalentClass>
        <rdfs:subClassOf rdf:resource="http://www.meteck.org/files/ontologies/stuff.owl#HomogeneousMixture"/>
        <rdfs:comment xml:lang="en">homogenous mixture with intermediate particle size. One stuff, the so-called &apos;dispersed medium&apos;, is microscopically dispersed evenly throughout another stuff, called the &apos;continuous medium&apos; (note: there&apos;s &gt;1 phase, whereas a solution has =1 phase; because of that, we cannot have colloid isa solution). Examples: milk, mayonaise, agar, fog

Colloids can be distinguished from solutions using the Tyndall effect. (A beam of light passing through a true solution is not visible, but light passing through a colloid will be reflected by the larger particles and the light beam will be visible.) 

it should be noted that the two stuffs are in a colloidFormingRelation. This is done separately over at the ContinuousMedium and DispersedPhase classes, because it is not inherent in the stuffs themselves.</rdfs:comment>
        <rdfs:comment>one can nag about the surfactants and stabilizers and enhancers. For instance, for whipping cream in homebaking, one can add the powder to keep the whipped cream stiff for longer (i.e., stabilise the colloid). </rdfs:comment>
    </owl:Class>
    


    <!-- http://www.meteck.org/files/ontologies/stuff.owl#Container -->

    <owl:Class rdf:about="http://www.meteck.org/files/ontologies/stuff.owl#Container">
        <rdfs:subClassOf rdf:resource="http://www.meteck.org/files/ontologies/stuff.owl#PhysicalEndurant"/>
        <rdfs:subClassOf>
            <owl:Restriction>
                <owl:onProperty>
                    <rdf:Description>
                        <owl:inverseOf rdf:resource="http://www.meteck.org/files/ontologies/stuff.owl#containedIn"/>
                    </rdf:Description>
                </owl:onProperty>
                <owl:allValuesFrom>
                    <owl:Class>
                        <owl:unionOf rdf:parseType="Collection">
                            <rdf:Description rdf:about="http://www.meteck.org/files/ontologies/stuff.owl#AmountOfStuff"/>
                            <rdf:Description rdf:about="http://www.meteck.org/files/ontologies/stuff.owl#PhysicalObject"/>
                        </owl:unionOf>
                    </owl:Class>
                </owl:allValuesFrom>
            </owl:Restriction>
        </rdfs:subClassOf>
        <rdfs:comment xml:lang="en">For if an amount of matter is not-selfcontained</rdfs:comment>
    </owl:Class>
    


    <!-- http://www.meteck.org/files/ontologies/stuff.owl#ContinuousMedium -->

    <owl:Class rdf:about="http://www.meteck.org/files/ontologies/stuff.owl#ContinuousMedium">
        <rdfs:subClassOf rdf:resource="http://www.meteck.org/files/ontologies/stuff.owl#StuffRole"/>
        <rdfs:subClassOf>
            <owl:Restriction>
                <owl:onProperty rdf:resource="http://www.meteck.org/files/ontologies/stuff.owl#colloidFormingRelation"/>
                <owl:someValuesFrom rdf:resource="http://www.meteck.org/files/ontologies/stuff.owl#DispersedPhase"/>
            </owl:Restriction>
        </rdfs:subClassOf>
        <owl:disjointWith rdf:resource="http://www.meteck.org/files/ontologies/stuff.owl#DispersedPhase"/>
        <rdfs:comment>also called dispersion medium</rdfs:comment>
    </owl:Class>
    


    <!-- http://www.meteck.org/files/ontologies/stuff.owl#DispersedPhase -->

    <owl:Class rdf:about="http://www.meteck.org/files/ontologies/stuff.owl#DispersedPhase">
        <rdfs:subClassOf rdf:resource="http://www.meteck.org/files/ontologies/stuff.owl#StuffRole"/>
        <rdfs:comment>the colloidFormingRelation is between the DispersedPhase and the ContinuousMedium and not their respective bearers (stuffs), because if you put the stuffs together just like that, you won&apos;t get the colloid; put differently, they have to be mixed in a particular way for it to become a homogenous mixture. E.g., opening a cup of cream and exposing it to an amount of air won&apos;t get you whipped cream, and putting the right amount of egg yolk and oil in the mixing bowl does not instantly become mayonnaise. It only work if the stuff that plays the role of dispersed phase is added gradually to the continuous medium in order to become a stable colloid. The same stuff can play eitehr role, depending on the colloid to be formed</rdfs:comment>
    </owl:Class>
    


    <!-- http://www.meteck.org/files/ontologies/stuff.owl#DispersionColloid -->

    <owl:Class rdf:about="http://www.meteck.org/files/ontologies/stuff.owl#DispersionColloid">
        <rdfs:subClassOf rdf:resource="http://www.meteck.org/files/ontologies/stuff.owl#Colloid"/>
        <rdfs:comment>the most common type of colloids (cf. the other two)</rdfs:comment>
    </owl:Class>
    


    <!-- http://www.meteck.org/files/ontologies/stuff.owl#Distribution -->

    <owl:Class rdf:about="http://www.meteck.org/files/ontologies/stuff.owl#Distribution">
        <rdfs:subClassOf rdf:resource="http://www.meteck.org/files/ontologies/stuff.owl#Quality"/>
        <rdfs:subClassOf>
            <owl:Restriction>
                <owl:onProperty rdf:resource="http://www.meteck.org/files/ontologies/stuff.owl#hasQuale"/>
                <owl:someValuesFrom>
                    <owl:Class>
                        <owl:unionOf rdf:parseType="Collection">
                            <rdf:Description rdf:about="http://www.meteck.org/files/ontologies/stuff.owl#EvenDistribution"/>
                            <rdf:Description rdf:about="http://www.meteck.org/files/ontologies/stuff.owl#UnevenDistribution"/>
                        </owl:unionOf>
                    </owl:Class>
                </owl:someValuesFrom>
            </owl:Restriction>
        </rdfs:subClassOf>
    </owl:Class>
    


    <!-- http://www.meteck.org/files/ontologies/stuff.owl#Drop -->

    <owl:Class rdf:about="http://www.meteck.org/files/ontologies/stuff.owl#Drop">
        <rdfs:subClassOf rdf:resource="http://www.meteck.org/files/ontologies/stuff.owl#Piece"/>
        <rdfs:comment xml:lang="en">type of a piece, added as example. e.g., a drop of blood</rdfs:comment>
    </owl:Class>
    


    <!-- http://www.meteck.org/files/ontologies/stuff.owl#Emulsion -->

    <owl:Class rdf:about="http://www.meteck.org/files/ontologies/stuff.owl#Emulsion">
        <owl:equivalentClass>
            <owl:Class>
                <owl:intersectionOf rdf:parseType="Collection">
                    <rdf:Description rdf:about="http://www.meteck.org/files/ontologies/stuff.owl#DispersionColloid"/>
                    <owl:Restriction>
                        <owl:onProperty rdf:resource="http://www.meteck.org/files/ontologies/stuff.owl#hasPartStuff"/>
                        <owl:qualifiedCardinality rdf:datatype="http://www.w3.org/2001/XMLSchema#nonNegativeInteger">1</owl:qualifiedCardinality>
                        <owl:onClass>
                            <owl:Class>
                                <owl:intersectionOf rdf:parseType="Collection">
                                    <rdf:Description rdf:about="http://www.meteck.org/files/ontologies/stuff.owl#Stuff"/>
                                    <owl:Restriction>
                                        <owl:onProperty rdf:resource="http://www.meteck.org/files/ontologies/stuff.owl#hasState"/>
                                        <owl:someValuesFrom rdf:resource="http://www.meteck.org/files/ontologies/stuff.owl#Liquid"/>
                                    </owl:Restriction>
                                    <owl:Restriction>
                                        <owl:onProperty>
                                            <rdf:Description>
                                                <owl:inverseOf rdf:resource="http://www.meteck.org/files/ontologies/stuff.owl#srInheresIn"/>
                                            </rdf:Description>
                                        </owl:onProperty>
                                        <owl:someValuesFrom rdf:resource="http://www.meteck.org/files/ontologies/stuff.owl#ContinuousMedium"/>
                                    </owl:Restriction>
                                </owl:intersectionOf>
                            </owl:Class>
                        </owl:onClass>
                    </owl:Restriction>
                    <owl:Restriction>
                        <owl:onProperty rdf:resource="http://www.meteck.org/files/ontologies/stuff.owl#hasPartStuff"/>
                        <owl:qualifiedCardinality rdf:datatype="http://www.w3.org/2001/XMLSchema#nonNegativeInteger">1</owl:qualifiedCardinality>
                        <owl:onClass>
                            <owl:Class>
                                <owl:intersectionOf rdf:parseType="Collection">
                                    <rdf:Description rdf:about="http://www.meteck.org/files/ontologies/stuff.owl#Stuff"/>
                                    <owl:Restriction>
                                        <owl:onProperty rdf:resource="http://www.meteck.org/files/ontologies/stuff.owl#hasState"/>
                                        <owl:someValuesFrom rdf:resource="http://www.meteck.org/files/ontologies/stuff.owl#Liquid"/>
                                    </owl:Restriction>
                                    <owl:Restriction>
                                        <owl:onProperty>
                                            <rdf:Description>
                                                <owl:inverseOf rdf:resource="http://www.meteck.org/files/ontologies/stuff.owl#srInheresIn"/>
                                            </rdf:Description>
                                        </owl:onProperty>
                                        <owl:someValuesFrom rdf:resource="http://www.meteck.org/files/ontologies/stuff.owl#DispersedPhase"/>
                                    </owl:Restriction>
                                </owl:intersectionOf>
                            </owl:Class>
                        </owl:onClass>
                    </owl:Restriction>
                </owl:intersectionOf>
            </owl:Class>
        </owl:equivalentClass>
        <rdfs:subClassOf rdf:resource="http://www.meteck.org/files/ontologies/stuff.owl#DispersionColloid"/>
        <rdfs:comment xml:lang="en">continuous medium: liquid
dispersed phase: liquid
Examples: milk, mayonnaise, hand cream
http://en.wikipedia.org/wiki/Colloid</rdfs:comment>
    </owl:Class>
    


    <!-- http://www.meteck.org/files/ontologies/stuff.owl#Endurant -->

    <owl:Class rdf:about="http://www.meteck.org/files/ontologies/stuff.owl#Endurant">
        <owl:disjointWith rdf:resource="http://www.meteck.org/files/ontologies/stuff.owl#Perdurant"/>
    </owl:Class>
    


    <!-- http://www.meteck.org/files/ontologies/stuff.owl#EvenDistribution -->

    <owl:Class rdf:about="http://www.meteck.org/files/ontologies/stuff.owl#EvenDistribution">
        <rdfs:subClassOf rdf:resource="http://www.meteck.org/files/ontologies/stuff.owl#AbstractRegion"/>
    </owl:Class>
    


    <!-- http://www.meteck.org/files/ontologies/stuff.owl#Foam -->

    <owl:Class rdf:about="http://www.meteck.org/files/ontologies/stuff.owl#Foam">
        <owl:equivalentClass>
            <owl:Class>
                <owl:intersectionOf rdf:parseType="Collection">
                    <rdf:Description rdf:about="http://www.meteck.org/files/ontologies/stuff.owl#DispersionColloid"/>
                    <owl:Restriction>
                        <owl:onProperty rdf:resource="http://www.meteck.org/files/ontologies/stuff.owl#hasPartStuff"/>
                        <owl:qualifiedCardinality rdf:datatype="http://www.w3.org/2001/XMLSchema#nonNegativeInteger">1</owl:qualifiedCardinality>
                        <owl:onClass>
                            <owl:Class>
                                <owl:intersectionOf rdf:parseType="Collection">
                                    <rdf:Description rdf:about="http://www.meteck.org/files/ontologies/stuff.owl#Stuff"/>
                                    <owl:Restriction>
                                        <owl:onProperty rdf:resource="http://www.meteck.org/files/ontologies/stuff.owl#hasState"/>
                                        <owl:someValuesFrom rdf:resource="http://www.meteck.org/files/ontologies/stuff.owl#Gas"/>
                                    </owl:Restriction>
                                    <owl:Restriction>
                                        <owl:onProperty>
                                            <rdf:Description>
                                                <owl:inverseOf rdf:resource="http://www.meteck.org/files/ontologies/stuff.owl#srInheresIn"/>
                                            </rdf:Description>
                                        </owl:onProperty>
                                        <owl:someValuesFrom rdf:resource="http://www.meteck.org/files/ontologies/stuff.owl#DispersedPhase"/>
                                    </owl:Restriction>
                                </owl:intersectionOf>
                            </owl:Class>
                        </owl:onClass>
                    </owl:Restriction>
                    <owl:Restriction>
                        <owl:onProperty rdf:resource="http://www.meteck.org/files/ontologies/stuff.owl#hasPartStuff"/>
                        <owl:qualifiedCardinality rdf:datatype="http://www.w3.org/2001/XMLSchema#nonNegativeInteger">1</owl:qualifiedCardinality>
                        <owl:onClass>
                            <owl:Class>
                                <owl:intersectionOf rdf:parseType="Collection">
                                    <rdf:Description rdf:about="http://www.meteck.org/files/ontologies/stuff.owl#Stuff"/>
                                    <owl:Restriction>
                                        <owl:onProperty rdf:resource="http://www.meteck.org/files/ontologies/stuff.owl#hasState"/>
                                        <owl:someValuesFrom rdf:resource="http://www.meteck.org/files/ontologies/stuff.owl#Liquid"/>
                                    </owl:Restriction>
                                    <owl:Restriction>
                                        <owl:onProperty>
                                            <rdf:Description>
                                                <owl:inverseOf rdf:resource="http://www.meteck.org/files/ontologies/stuff.owl#srInheresIn"/>
                                            </rdf:Description>
                                        </owl:onProperty>
                                        <owl:someValuesFrom rdf:resource="http://www.meteck.org/files/ontologies/stuff.owl#ContinuousMedium"/>
                                    </owl:Restriction>
                                </owl:intersectionOf>
                            </owl:Class>
                        </owl:onClass>
                    </owl:Restriction>
                </owl:intersectionOf>
            </owl:Class>
        </owl:equivalentClass>
        <rdfs:subClassOf rdf:resource="http://www.meteck.org/files/ontologies/stuff.owl#DispersionColloid"/>
        <rdfs:comment xml:lang="en">continuous medium: liquid
dispersed phase: gas
Examples: whipped cream, shaving cream
http://en.wikipedia.org/wiki/Colloid</rdfs:comment>
    </owl:Class>
    


    <!-- http://www.meteck.org/files/ontologies/stuff.owl#Gas -->

    <owl:Class rdf:about="http://www.meteck.org/files/ontologies/stuff.owl#Gas">
        <rdfs:subClassOf rdf:resource="http://www.meteck.org/files/ontologies/stuff.owl#StuffState"/>
    </owl:Class>
    


    <!-- http://www.meteck.org/files/ontologies/stuff.owl#Gel -->

    <owl:Class rdf:about="http://www.meteck.org/files/ontologies/stuff.owl#Gel">
        <owl:equivalentClass>
            <owl:Class>
                <owl:intersectionOf rdf:parseType="Collection">
                    <rdf:Description rdf:about="http://www.meteck.org/files/ontologies/stuff.owl#DispersionColloid"/>
                    <owl:Restriction>
                        <owl:onProperty rdf:resource="http://www.meteck.org/files/ontologies/stuff.owl#hasPartStuff"/>
                        <owl:qualifiedCardinality rdf:datatype="http://www.w3.org/2001/XMLSchema#nonNegativeInteger">1</owl:qualifiedCardinality>
                        <owl:onClass>
                            <owl:Class>
                                <owl:intersectionOf rdf:parseType="Collection">
                                    <rdf:Description rdf:about="http://www.meteck.org/files/ontologies/stuff.owl#Stuff"/>
                                    <owl:Restriction>
                                        <owl:onProperty rdf:resource="http://www.meteck.org/files/ontologies/stuff.owl#hasState"/>
                                        <owl:someValuesFrom rdf:resource="http://www.meteck.org/files/ontologies/stuff.owl#Liquid"/>
                                    </owl:Restriction>
                                    <owl:Restriction>
                                        <owl:onProperty>
                                            <rdf:Description>
                                                <owl:inverseOf rdf:resource="http://www.meteck.org/files/ontologies/stuff.owl#srInheresIn"/>
                                            </rdf:Description>
                                        </owl:onProperty>
                                        <owl:someValuesFrom rdf:resource="http://www.meteck.org/files/ontologies/stuff.owl#DispersedPhase"/>
                                    </owl:Restriction>
                                </owl:intersectionOf>
                            </owl:Class>
                        </owl:onClass>
                    </owl:Restriction>
                    <owl:Restriction>
                        <owl:onProperty rdf:resource="http://www.meteck.org/files/ontologies/stuff.owl#hasPartStuff"/>
                        <owl:qualifiedCardinality rdf:datatype="http://www.w3.org/2001/XMLSchema#nonNegativeInteger">1</owl:qualifiedCardinality>
                        <owl:onClass>
                            <owl:Class>
                                <owl:intersectionOf rdf:parseType="Collection">
                                    <rdf:Description rdf:about="http://www.meteck.org/files/ontologies/stuff.owl#Stuff"/>
                                    <owl:Restriction>
                                        <owl:onProperty rdf:resource="http://www.meteck.org/files/ontologies/stuff.owl#hasState"/>
                                        <owl:someValuesFrom rdf:resource="http://www.meteck.org/files/ontologies/stuff.owl#Solid"/>
                                    </owl:Restriction>
                                    <owl:Restriction>
                                        <owl:onProperty>
                                            <rdf:Description>
                                                <owl:inverseOf rdf:resource="http://www.meteck.org/files/ontologies/stuff.owl#srInheresIn"/>
                                            </rdf:Description>
                                        </owl:onProperty>
                                        <owl:someValuesFrom rdf:resource="http://www.meteck.org/files/ontologies/stuff.owl#ContinuousMedium"/>
                                    </owl:Restriction>
                                </owl:intersectionOf>
                            </owl:Class>
                        </owl:onClass>
                    </owl:Restriction>
                </owl:intersectionOf>
            </owl:Class>
        </owl:equivalentClass>
        <rdfs:subClassOf rdf:resource="http://www.meteck.org/files/ontologies/stuff.owl#DispersionColloid"/>
        <rdfs:comment xml:lang="en">continuous medium: solid
dispersed phase: liquid
Examples: agar, gelatin, jelly
http://en.wikipedia.org/wiki/Colloid </rdfs:comment>
    </owl:Class>
    


    <!-- http://www.meteck.org/files/ontologies/stuff.owl#HeterogeneousMixture -->

    <owl:Class rdf:about="http://www.meteck.org/files/ontologies/stuff.owl#HeterogeneousMixture">
        <rdfs:subClassOf rdf:resource="http://www.meteck.org/files/ontologies/stuff.owl#MixedStuff"/>
        <rdfs:subClassOf>
            <owl:Restriction>
                <owl:onProperty rdf:resource="http://www.meteck.org/files/ontologies/stuff.owl#hasGranuleType"/>
                <owl:minQualifiedCardinality rdf:datatype="http://www.w3.org/2001/XMLSchema#nonNegativeInteger">2</owl:minQualifiedCardinality>
                <owl:onClass>
                    <owl:Class>
                        <owl:unionOf rdf:parseType="Collection">
                            <rdf:Description rdf:about="http://www.meteck.org/files/ontologies/stuff.owl#Molecule"/>
                            <rdf:Description rdf:about="http://www.meteck.org/files/ontologies/stuff.owl#MultiMoleculeParticle"/>
                        </owl:unionOf>
                    </owl:Class>
                </owl:onClass>
            </owl:Restriction>
        </rdfs:subClassOf>
        <rdfs:subClassOf>
            <owl:Restriction>
                <owl:onProperty rdf:resource="http://www.meteck.org/files/ontologies/stuff.owl#hasPartStuff"/>
                <owl:minQualifiedCardinality rdf:datatype="http://www.w3.org/2001/XMLSchema#nonNegativeInteger">2</owl:minQualifiedCardinality>
                <owl:onClass>
                    <owl:Class>
                        <owl:unionOf rdf:parseType="Collection">
                            <rdf:Description rdf:about="http://www.meteck.org/files/ontologies/stuff.owl#MixedStuff"/>
                            <rdf:Description rdf:about="http://www.meteck.org/files/ontologies/stuff.owl#PureStuff"/>
                        </owl:unionOf>
                    </owl:Class>
                </owl:onClass>
            </owl:Restriction>
        </rdfs:subClassOf>
        <rdfs:subClassOf>
            <owl:Restriction>
                <owl:onProperty rdf:resource="http://www.meteck.org/files/ontologies/stuff.owl#hasStuffDistribution"/>
                <owl:qualifiedCardinality rdf:datatype="http://www.w3.org/2001/XMLSchema#nonNegativeInteger">1</owl:qualifiedCardinality>
                <owl:onClass rdf:resource="http://www.meteck.org/files/ontologies/stuff.owl#UnevenDistribution"/>
            </owl:Restriction>
        </rdfs:subClassOf>
        <owl:disjointWith rdf:resource="http://www.meteck.org/files/ontologies/stuff.owl#HomogeneousMixture"/>
        <rdfs:comment xml:lang="en">Combination of different stuffs (of which at least one with a fairly large particle size) that don&apos;t react, and can be separated by purely physical means (filtration, etc). Contrast with homogenously mixed stuffs like colloids and solutions where its components are evenly distributed across the stuff. portion in the sense of taking a &apos;part&apos;/section of this heterogenous stuff, then it generally is the case that the subquantity is not of the same stuffkind as the whole quantity, only when the portion is carefully constructed and the so-called stuff-forming relation still holds.</rdfs:comment>
    </owl:Class>
    


    <!-- http://www.meteck.org/files/ontologies/stuff.owl#HomogeneousMixture -->

    <owl:Class rdf:about="http://www.meteck.org/files/ontologies/stuff.owl#HomogeneousMixture">
        <rdfs:subClassOf rdf:resource="http://www.meteck.org/files/ontologies/stuff.owl#MixedStuff"/>
        <rdfs:subClassOf>
            <owl:Restriction>
                <owl:onProperty rdf:resource="http://www.meteck.org/files/ontologies/stuff.owl#hasGranuleType"/>
                <owl:allValuesFrom>
                    <owl:Class>
                        <owl:unionOf rdf:parseType="Collection">
                            <rdf:Description rdf:about="http://www.meteck.org/files/ontologies/stuff.owl#Atom"/>
                            <rdf:Description rdf:about="http://www.meteck.org/files/ontologies/stuff.owl#Ion"/>
                            <rdf:Description rdf:about="http://www.meteck.org/files/ontologies/stuff.owl#Molecule"/>
                        </owl:unionOf>
                    </owl:Class>
                </owl:allValuesFrom>
            </owl:Restriction>
        </rdfs:subClassOf>
        <rdfs:subClassOf>
            <owl:Restriction>
                <owl:onProperty rdf:resource="http://www.meteck.org/files/ontologies/stuff.owl#hasStuffDistribution"/>
                <owl:qualifiedCardinality rdf:datatype="http://www.w3.org/2001/XMLSchema#nonNegativeInteger">1</owl:qualifiedCardinality>
                <owl:onClass rdf:resource="http://www.meteck.org/files/ontologies/stuff.owl#EvenDistribution"/>
            </owl:Restriction>
        </rdfs:subClassOf>
        <rdfs:comment>the mixed stuffs are evenly distributed across the amount of matter (macroscopic sameness). Some would call only a solution a homogeneous mixture, not colloids, because solutions have one phase only, whereas colloids have at least 2. We take an inclusive approach here, and refine further in the two subclasses.</rdfs:comment>
    </owl:Class>
    


    <!-- http://www.meteck.org/files/ontologies/stuff.owl#Ion -->

    <owl:Class rdf:about="http://www.meteck.org/files/ontologies/stuff.owl#Ion">
        <rdfs:subClassOf rdf:resource="http://www.meteck.org/files/ontologies/stuff.owl#PhysicalObject"/>
    </owl:Class>
    


    <!-- http://www.meteck.org/files/ontologies/stuff.owl#LeastPortion -->

    <owl:Class rdf:about="http://www.meteck.org/files/ontologies/stuff.owl#LeastPortion">
        <rdfs:subClassOf rdf:resource="http://www.meteck.org/files/ontologies/stuff.owl#Portion"/>
        <rdfs:subClassOf>
            <owl:Class>
                <owl:complementOf>
                    <owl:Restriction>
                        <owl:onProperty rdf:resource="http://www.meteck.org/files/ontologies/stuff.owl#hasPortion"/>
                        <owl:someValuesFrom rdf:resource="http://www.meteck.org/files/ontologies/stuff.owl#Portion"/>
                    </owl:Restriction>
                </owl:complementOf>
            </owl:Class>
        </rdfs:subClassOf>
        <rdfs:comment xml:lang="en">The smallest portion that still exhibits the macroscopic properties of that kind of stuff. like Atom in merology, but then for stuffs.</rdfs:comment>
    </owl:Class>
    


    <!-- http://www.meteck.org/files/ontologies/stuff.owl#Liquid -->

    <owl:Class rdf:about="http://www.meteck.org/files/ontologies/stuff.owl#Liquid">
        <rdfs:subClassOf rdf:resource="http://www.meteck.org/files/ontologies/stuff.owl#StuffState"/>
    </owl:Class>
    


    <!-- http://www.meteck.org/files/ontologies/stuff.owl#LiquidAerosol -->

    <owl:Class rdf:about="http://www.meteck.org/files/ontologies/stuff.owl#LiquidAerosol">
        <owl:equivalentClass>
            <owl:Class>
                <owl:intersectionOf rdf:parseType="Collection">
                    <rdf:Description rdf:about="http://www.meteck.org/files/ontologies/stuff.owl#DispersionColloid"/>
                    <owl:Restriction>
                        <owl:onProperty rdf:resource="http://www.meteck.org/files/ontologies/stuff.owl#hasPartStuff"/>
                        <owl:qualifiedCardinality rdf:datatype="http://www.w3.org/2001/XMLSchema#nonNegativeInteger">1</owl:qualifiedCardinality>
                        <owl:onClass>
                            <owl:Class>
                                <owl:intersectionOf rdf:parseType="Collection">
                                    <rdf:Description rdf:about="http://www.meteck.org/files/ontologies/stuff.owl#Stuff"/>
                                    <owl:Restriction>
                                        <owl:onProperty rdf:resource="http://www.meteck.org/files/ontologies/stuff.owl#hasState"/>
                                        <owl:someValuesFrom rdf:resource="http://www.meteck.org/files/ontologies/stuff.owl#Gas"/>
                                    </owl:Restriction>
                                    <owl:Restriction>
                                        <owl:onProperty>
                                            <rdf:Description>
                                                <owl:inverseOf rdf:resource="http://www.meteck.org/files/ontologies/stuff.owl#srInheresIn"/>
                                            </rdf:Description>
                                        </owl:onProperty>
                                        <owl:someValuesFrom rdf:resource="http://www.meteck.org/files/ontologies/stuff.owl#ContinuousMedium"/>
                                    </owl:Restriction>
                                </owl:intersectionOf>
                            </owl:Class>
                        </owl:onClass>
                    </owl:Restriction>
                    <owl:Restriction>
                        <owl:onProperty rdf:resource="http://www.meteck.org/files/ontologies/stuff.owl#hasPartStuff"/>
                        <owl:qualifiedCardinality rdf:datatype="http://www.w3.org/2001/XMLSchema#nonNegativeInteger">1</owl:qualifiedCardinality>
                        <owl:onClass>
                            <owl:Class>
                                <owl:intersectionOf rdf:parseType="Collection">
                                    <rdf:Description rdf:about="http://www.meteck.org/files/ontologies/stuff.owl#Stuff"/>
                                    <owl:Restriction>
                                        <owl:onProperty rdf:resource="http://www.meteck.org/files/ontologies/stuff.owl#hasState"/>
                                        <owl:someValuesFrom rdf:resource="http://www.meteck.org/files/ontologies/stuff.owl#Liquid"/>
                                    </owl:Restriction>
                                    <owl:Restriction>
                                        <owl:onProperty>
                                            <rdf:Description>
                                                <owl:inverseOf rdf:resource="http://www.meteck.org/files/ontologies/stuff.owl#srInheresIn"/>
                                            </rdf:Description>
                                        </owl:onProperty>
                                        <owl:someValuesFrom rdf:resource="http://www.meteck.org/files/ontologies/stuff.owl#DispersedPhase"/>
                                    </owl:Restriction>
                                </owl:intersectionOf>
                            </owl:Class>
                        </owl:onClass>
                    </owl:Restriction>
                </owl:intersectionOf>
            </owl:Class>
        </owl:equivalentClass>
        <rdfs:subClassOf rdf:resource="http://www.meteck.org/files/ontologies/stuff.owl#DispersionColloid"/>
        <rdfs:comment xml:lang="en">continuous medium: gas
dispersed phase: liquid
Examples: fog mist, hair sprays
http://en.wikipedia.org/wiki/Colloid</rdfs:comment>
    </owl:Class>
    


    <!-- http://www.meteck.org/files/ontologies/stuff.owl#Lump -->

    <owl:Class rdf:about="http://www.meteck.org/files/ontologies/stuff.owl#Lump">
        <rdfs:subClassOf rdf:resource="http://www.meteck.org/files/ontologies/stuff.owl#Piece"/>
        <rdfs:comment xml:lang="en">type of a piece, added as example. e.g., lump of clay</rdfs:comment>
    </owl:Class>
    


    <!-- http://www.meteck.org/files/ontologies/stuff.owl#MicellarColloid -->

    <owl:Class rdf:about="http://www.meteck.org/files/ontologies/stuff.owl#MicellarColloid">
        <rdfs:subClassOf rdf:resource="http://www.meteck.org/files/ontologies/stuff.owl#AssociationalColloid"/>
        <rdfs:comment>A careful reader will observe tehre is no distinction between this and the Associational colloid. The distinction is largely due to terminology in food physics and physics &amp; colloid chemistry.</rdfs:comment>
    </owl:Class>
    


    <!-- http://www.meteck.org/files/ontologies/stuff.owl#MixedStuff -->

    <owl:Class rdf:about="http://www.meteck.org/files/ontologies/stuff.owl#MixedStuff">
        <rdfs:subClassOf rdf:resource="http://www.meteck.org/files/ontologies/stuff.owl#Stuff"/>
        <rdfs:subClassOf>
            <owl:Class>
                <owl:intersectionOf rdf:parseType="Collection">
                    <rdf:Description rdf:about="http://www.meteck.org/files/ontologies/stuff.owl#Stuff"/>
                    <owl:Restriction>
                        <owl:onProperty rdf:resource="http://www.meteck.org/files/ontologies/stuff.owl#hasPartStuff"/>
                        <owl:minQualifiedCardinality rdf:datatype="http://www.w3.org/2001/XMLSchema#nonNegativeInteger">2</owl:minQualifiedCardinality>
                        <owl:onClass rdf:resource="http://www.meteck.org/files/ontologies/stuff.owl#Stuff"/>
                    </owl:Restriction>
                </owl:intersectionOf>
            </owl:Class>
        </rdfs:subClassOf>
        <owl:disjointWith rdf:resource="http://www.meteck.org/files/ontologies/stuff.owl#PureStuff"/>
        <owl:disjointUnionOf rdf:parseType="Collection">
            <rdf:Description rdf:about="http://www.meteck.org/files/ontologies/stuff.owl#HeterogeneousMixture"/>
            <rdf:Description rdf:about="http://www.meteck.org/files/ontologies/stuff.owl#HomogeneousMixture"/>
        </owl:disjointUnionOf>
        <rdfs:comment>Core differences between mixtures and compouds: the proportions of the components may vary, the individual components are observable, and the components can be separated by physical means. [Silberberg, 4th ed, p73]</rdfs:comment>
        <rdfs:comment>Note: categorisation according to components, with their role. We do not include &apos;phase mixtures&apos;, like having an ice cube (solid water) in a glass of liquid water; in that case, it is still the pure stuff water. 
For colloids, one does have to take into account the state of the stuff to define different kinds of colloids, but the point is that they are composed of different kinds of stuff. </rdfs:comment>
    </owl:Class>
    


    <!-- http://www.meteck.org/files/ontologies/stuff.owl#MolecularColloid -->

    <owl:Class rdf:about="http://www.meteck.org/files/ontologies/stuff.owl#MolecularColloid">
        <rdfs:subClassOf rdf:resource="http://www.meteck.org/files/ontologies/stuff.owl#Colloid"/>
        <rdfs:comment>Colloid where the molecules are so big they have the behaviour of that of the intermediate particle size in the other colloids.
Example: latex (and other starchy things, with big polymers)</rdfs:comment>
    </owl:Class>
    


    <!-- http://www.meteck.org/files/ontologies/stuff.owl#Molecule -->

    <owl:Class rdf:about="http://www.meteck.org/files/ontologies/stuff.owl#Molecule">
        <rdfs:subClassOf rdf:resource="http://www.meteck.org/files/ontologies/stuff.owl#PhysicalObject"/>
        <rdfs:subClassOf>
            <owl:Restriction>
                <owl:onProperty rdf:resource="http://www.meteck.org/files/ontologies/stuff.owl#hasPart"/>
                <owl:someValuesFrom rdf:resource="http://www.meteck.org/files/ontologies/stuff.owl#Atom"/>
            </owl:Restriction>
        </rdfs:subClassOf>
        <rdfs:comment xml:lang="en">The instances of this class are sort of a hack so as to stay within first order logc. Strictly speaking, the molecues that are here included as example are classes, not individuals (an individual H2O molecule in your body is), but typically we do not care about one individual such molecule. also, putting them as indivisuals in the ontology, when we have, say, hasConstituent =1 Molecule, we&apos;re actually talking of type of molecule, not an individual one. but pushing everything one level down, we get the desired behaviour of the reasoner....</rdfs:comment>
        <rdfs:comment>has as part two or more chemically bonded atoms (but if I say &gt;=2 in the axiom, then it&apos;s not simple anymore, adn have to give up transitivity, which I don&apos;t want to)</rdfs:comment>
    </owl:Class>
    


    <!-- http://www.meteck.org/files/ontologies/stuff.owl#MultiMoleculeParticle -->

    <owl:Class rdf:about="http://www.meteck.org/files/ontologies/stuff.owl#MultiMoleculeParticle">
        <rdfs:subClassOf rdf:resource="http://www.meteck.org/files/ontologies/stuff.owl#PhysicalObject"/>
        <rdfs:comment>Multi-molecular particle, like those in a suspension, the droplets in a colloid (i.e, not the sub-atomic particles)</rdfs:comment>
        <rdfs:comment xml:lang="en">see annotation to Molecule that this class&apos; instances is a bit of a hack.</rdfs:comment>
    </owl:Class>
    


    <!-- http://www.meteck.org/files/ontologies/stuff.owl#NumberOfPhases -->

    <owl:Class rdf:about="http://www.meteck.org/files/ontologies/stuff.owl#NumberOfPhases">
        <rdfs:subClassOf rdf:resource="http://www.meteck.org/files/ontologies/stuff.owl#AbstractRegion"/>
        <rdfs:subClassOf>
            <owl:Restriction>
                <owl:onProperty rdf:resource="http://www.meteck.org/files/ontologies/stuff.owl#hasDataValue"/>
                <owl:someValuesFrom rdf:resource="http://www.w3.org/2001/XMLSchema#nonNegativeInteger"/>
            </owl:Restriction>
        </rdfs:subClassOf>
        <rdfs:comment>alternative way of modelling the number of phases, the other one being with the data type</rdfs:comment>
    </owl:Class>
    


    <!-- http://www.meteck.org/files/ontologies/stuff.owl#Paste -->

    <owl:Class rdf:about="http://www.meteck.org/files/ontologies/stuff.owl#Paste">
        <rdfs:subClassOf rdf:resource="http://www.meteck.org/files/ontologies/stuff.owl#Suspension"/>
        <rdfs:comment>suspension with less dispersion medium and the dispersed phase is connected</rdfs:comment>
    </owl:Class>
    


    <!-- http://www.meteck.org/files/ontologies/stuff.owl#Perdurant -->

    <owl:Class rdf:about="http://www.meteck.org/files/ontologies/stuff.owl#Perdurant"/>
    


    <!-- http://www.meteck.org/files/ontologies/stuff.owl#PhysicalEndurant -->

    <owl:Class rdf:about="http://www.meteck.org/files/ontologies/stuff.owl#PhysicalEndurant">
        <owl:equivalentClass rdf:resource="http://www.wurvoc.org/vocabularies/om-1.8/Phenomenon"/>
        <rdfs:subClassOf rdf:resource="http://www.meteck.org/files/ontologies/stuff.owl#Endurant"/>
        <owl:disjointWith rdf:resource="http://www.meteck.org/files/ontologies/stuff.owl#Role"/>
    </owl:Class>
    


    <!-- http://www.meteck.org/files/ontologies/stuff.owl#PhysicalObject -->

    <owl:Class rdf:about="http://www.meteck.org/files/ontologies/stuff.owl#PhysicalObject">
        <rdfs:subClassOf rdf:resource="http://www.meteck.org/files/ontologies/stuff.owl#PhysicalEndurant"/>
        <owl:disjointWith rdf:resource="http://www.meteck.org/files/ontologies/stuff.owl#Stuff"/>
    </owl:Class>
    


    <!-- http://www.meteck.org/files/ontologies/stuff.owl#PhysicalRegion -->

    <owl:Class rdf:about="http://www.meteck.org/files/ontologies/stuff.owl#PhysicalRegion">
        <rdfs:subClassOf rdf:resource="http://www.meteck.org/files/ontologies/stuff.owl#Region"/>
    </owl:Class>
    


    <!-- http://www.meteck.org/files/ontologies/stuff.owl#Piece -->

    <owl:Class rdf:about="http://www.meteck.org/files/ontologies/stuff.owl#Piece">
        <rdfs:subClassOf rdf:resource="http://www.meteck.org/files/ontologies/stuff.owl#Portion"/>
        <rdfs:subClassOf>
            <owl:Restriction>
                <owl:onProperty rdf:resource="http://www.meteck.org/files/ontologies/stuff.owl#isSelfContainedScatteredPortionOf"/>
                <owl:someValuesFrom rdf:resource="http://www.meteck.org/files/ontologies/stuff.owl#AmountOfStuff"/>
            </owl:Restriction>
        </rdfs:subClassOf>
        <rdfs:comment xml:lang="en">self-contained amounts, like slices, lumps, etc. Only three subcalsses are added, for illustration, but feel free to add more.</rdfs:comment>
    </owl:Class>
    


    <!-- http://www.meteck.org/files/ontologies/stuff.owl#Portion -->

    <owl:Class rdf:about="http://www.meteck.org/files/ontologies/stuff.owl#Portion">
        <rdfs:subClassOf rdf:resource="http://www.meteck.org/files/ontologies/stuff.owl#AmountOfStuff"/>
        <rdfs:subClassOf>
            <owl:Restriction>
                <owl:onProperty rdf:resource="http://www.meteck.org/files/ontologies/stuff.owl#portionOf"/>
                <owl:someValuesFrom rdf:resource="http://www.meteck.org/files/ontologies/stuff.owl#AmountOfStuff"/>
            </owl:Restriction>
        </rdfs:subClassOf>
    </owl:Class>
    


    <!-- http://www.meteck.org/files/ontologies/stuff.owl#PureBulk -->

    <owl:Class rdf:about="http://www.meteck.org/files/ontologies/stuff.owl#PureBulk">
        <owl:equivalentClass>
            <owl:Class>
                <owl:intersectionOf rdf:parseType="Collection">
                    <rdf:Description rdf:about="http://www.meteck.org/files/ontologies/stuff.owl#PureStuff"/>
                    <owl:Restriction>
                        <owl:onProperty rdf:resource="http://www.meteck.org/files/ontologies/stuff.owl#hasGranuleType"/>
                        <owl:allValuesFrom rdf:resource="http://www.meteck.org/files/ontologies/stuff.owl#MultiMoleculeParticle"/>
                    </owl:Restriction>
                    <owl:Restriction>
                        <owl:onProperty rdf:resource="http://www.meteck.org/files/ontologies/stuff.owl#hasGranuleType"/>
                        <owl:qualifiedCardinality rdf:datatype="http://www.w3.org/2001/XMLSchema#nonNegativeInteger">1</owl:qualifiedCardinality>
                        <owl:onClass rdf:resource="http://www.meteck.org/files/ontologies/stuff.owl#MultiMoleculeParticle"/>
                    </owl:Restriction>
                </owl:intersectionOf>
            </owl:Class>
        </owl:equivalentClass>
        <rdfs:subClassOf rdf:resource="http://www.meteck.org/files/ontologies/stuff.owl#PureStuff"/>
        <rdfs:comment>difference with StructuredPureStuff and UnstructuredPureStuff: basis type, which is a multi-molecular object/particle.
Examples: a silo of soy beans, a packet of tea biscuits, a bag of cashew nuts</rdfs:comment>
        <rdfs:comment>there should be a &apos;has basis type exactly *one type of* multimoleculeparticle&apos; , not just one single individual multimoleculeparticle.</rdfs:comment>
    </owl:Class>
    


    <!-- http://www.meteck.org/files/ontologies/stuff.owl#PureStuff -->

    <owl:Class rdf:about="http://www.meteck.org/files/ontologies/stuff.owl#PureStuff">
        <owl:equivalentClass>
            <owl:Class>
                <owl:intersectionOf rdf:parseType="Collection">
                    <rdf:Description rdf:about="http://www.meteck.org/files/ontologies/stuff.owl#Stuff"/>
                    <owl:Restriction>
                        <owl:onProperty rdf:resource="http://www.meteck.org/files/ontologies/stuff.owl#hasGranuleType"/>
                        <owl:qualifiedCardinality rdf:datatype="http://www.w3.org/2001/XMLSchema#nonNegativeInteger">1</owl:qualifiedCardinality>
                        <owl:onClass>
                            <owl:Class>
                                <owl:unionOf rdf:parseType="Collection">
                                    <rdf:Description rdf:about="http://www.meteck.org/files/ontologies/stuff.owl#Atom"/>
                                    <rdf:Description rdf:about="http://www.meteck.org/files/ontologies/stuff.owl#Molecule"/>
                                    <rdf:Description rdf:about="http://www.meteck.org/files/ontologies/stuff.owl#MultiMoleculeParticle"/>
                                </owl:unionOf>
                            </owl:Class>
                        </owl:onClass>
                    </owl:Restriction>
                    <owl:Restriction>
                        <owl:onProperty rdf:resource="http://www.meteck.org/files/ontologies/stuff.owl#hasPartStuff"/>
                        <owl:qualifiedCardinality rdf:datatype="http://www.w3.org/2001/XMLSchema#nonNegativeInteger">1</owl:qualifiedCardinality>
                        <owl:onClass>
                            <owl:Class>
                                <owl:unionOf rdf:parseType="Collection">
                                    <rdf:Description rdf:about="http://www.meteck.org/files/ontologies/stuff.owl#PureBulk"/>
                                    <rdf:Description rdf:about="http://www.meteck.org/files/ontologies/stuff.owl#StructuredPureStuff"/>
                                    <rdf:Description rdf:about="http://www.meteck.org/files/ontologies/stuff.owl#UnstructuredPureStuff"/>
                                </owl:unionOf>
                            </owl:Class>
                        </owl:onClass>
                    </owl:Restriction>
                    <owl:Restriction>
                        <owl:onProperty rdf:resource="http://www.meteck.org/files/ontologies/stuff.owl#hasStuffDistribution"/>
                        <owl:qualifiedCardinality rdf:datatype="http://www.w3.org/2001/XMLSchema#nonNegativeInteger">1</owl:qualifiedCardinality>
                        <owl:onClass rdf:resource="http://www.meteck.org/files/ontologies/stuff.owl#EvenDistribution"/>
                    </owl:Restriction>
                </owl:intersectionOf>
            </owl:Class>
        </owl:equivalentClass>
        <rdfs:subClassOf rdf:resource="http://www.meteck.org/files/ontologies/stuff.owl#Stuff"/>
        <owl:disjointUnionOf rdf:parseType="Collection">
            <rdf:Description rdf:about="http://www.meteck.org/files/ontologies/stuff.owl#PureBulk"/>
            <rdf:Description rdf:about="http://www.meteck.org/files/ontologies/stuff.owl#StructuredPureStuff"/>
            <rdf:Description rdf:about="http://www.meteck.org/files/ontologies/stuff.owl#UnstructuredPureStuff"/>
        </owl:disjointUnionOf>
        <rdfs:comment xml:lang="en">Called &apos;Unstructed stuff&apos; in Donnelly &amp; Bittner, Phil Stud, 2009, and &apos;discrete stuff&apos; by Barnett, Phil Rev, 2004. They are refined here.</rdfs:comment>
        <rdfs:comment xml:lang="en">Composed of the same kind of molecules. For instance, Water, which consists of H2O molecules only, Alcohol, consisting of ethanol molecules only, etc, manganese and likewise for the other elements. 
This primarily serves as a useful theoretical category, i.e., it is an idealised case, as in reality the &apos;pure stuffs&apos; are only pure with respect to the measuring device with which one would be able to detect an impurity.</rdfs:comment>
    </owl:Class>
    


    <!-- http://www.meteck.org/files/ontologies/stuff.owl#Quality -->

    <owl:Class rdf:about="http://www.meteck.org/files/ontologies/stuff.owl#Quality"/>
    


    <!-- http://www.meteck.org/files/ontologies/stuff.owl#Region -->

    <owl:Class rdf:about="http://www.meteck.org/files/ontologies/stuff.owl#Region">
        <rdfs:subClassOf rdf:resource="http://www.meteck.org/files/ontologies/stuff.owl#Abstract"/>
    </owl:Class>
    


    <!-- http://www.meteck.org/files/ontologies/stuff.owl#Role -->

    <owl:Class rdf:about="http://www.meteck.org/files/ontologies/stuff.owl#Role">
        <rdfs:subClassOf rdf:resource="http://www.meteck.org/files/ontologies/stuff.owl#Endurant"/>
    </owl:Class>
    


    <!-- http://www.meteck.org/files/ontologies/stuff.owl#Slice -->

    <owl:Class rdf:about="http://www.meteck.org/files/ontologies/stuff.owl#Slice">
        <rdfs:subClassOf rdf:resource="http://www.meteck.org/files/ontologies/stuff.owl#Piece"/>
        <rdfs:comment xml:lang="en">type of a piece, added as example. e.g., slice of bread</rdfs:comment>
    </owl:Class>
    


    <!-- http://www.meteck.org/files/ontologies/stuff.owl#Sol -->

    <owl:Class rdf:about="http://www.meteck.org/files/ontologies/stuff.owl#Sol">
        <owl:equivalentClass>
            <owl:Class>
                <owl:intersectionOf rdf:parseType="Collection">
                    <rdf:Description rdf:about="http://www.meteck.org/files/ontologies/stuff.owl#DispersionColloid"/>
                    <owl:Restriction>
                        <owl:onProperty rdf:resource="http://www.meteck.org/files/ontologies/stuff.owl#hasPartStuff"/>
                        <owl:qualifiedCardinality rdf:datatype="http://www.w3.org/2001/XMLSchema#nonNegativeInteger">1</owl:qualifiedCardinality>
                        <owl:onClass>
                            <owl:Class>
                                <owl:intersectionOf rdf:parseType="Collection">
                                    <rdf:Description rdf:about="http://www.meteck.org/files/ontologies/stuff.owl#Stuff"/>
                                    <owl:Restriction>
                                        <owl:onProperty rdf:resource="http://www.meteck.org/files/ontologies/stuff.owl#hasState"/>
                                        <owl:someValuesFrom rdf:resource="http://www.meteck.org/files/ontologies/stuff.owl#Liquid"/>
                                    </owl:Restriction>
                                    <owl:Restriction>
                                        <owl:onProperty>
                                            <rdf:Description>
                                                <owl:inverseOf rdf:resource="http://www.meteck.org/files/ontologies/stuff.owl#srInheresIn"/>
                                            </rdf:Description>
                                        </owl:onProperty>
                                        <owl:someValuesFrom rdf:resource="http://www.meteck.org/files/ontologies/stuff.owl#ContinuousMedium"/>
                                    </owl:Restriction>
                                </owl:intersectionOf>
                            </owl:Class>
                        </owl:onClass>
                    </owl:Restriction>
                    <owl:Restriction>
                        <owl:onProperty rdf:resource="http://www.meteck.org/files/ontologies/stuff.owl#hasPartStuff"/>
                        <owl:qualifiedCardinality rdf:datatype="http://www.w3.org/2001/XMLSchema#nonNegativeInteger">1</owl:qualifiedCardinality>
                        <owl:onClass>
                            <owl:Class>
                                <owl:intersectionOf rdf:parseType="Collection">
                                    <rdf:Description rdf:about="http://www.meteck.org/files/ontologies/stuff.owl#Stuff"/>
                                    <owl:Restriction>
                                        <owl:onProperty rdf:resource="http://www.meteck.org/files/ontologies/stuff.owl#hasState"/>
                                        <owl:someValuesFrom rdf:resource="http://www.meteck.org/files/ontologies/stuff.owl#Solid"/>
                                    </owl:Restriction>
                                    <owl:Restriction>
                                        <owl:onProperty>
                                            <rdf:Description>
                                                <owl:inverseOf rdf:resource="http://www.meteck.org/files/ontologies/stuff.owl#srInheresIn"/>
                                            </rdf:Description>
                                        </owl:onProperty>
                                        <owl:someValuesFrom rdf:resource="http://www.meteck.org/files/ontologies/stuff.owl#DispersedPhase"/>
                                    </owl:Restriction>
                                </owl:intersectionOf>
                            </owl:Class>
                        </owl:onClass>
                    </owl:Restriction>
                </owl:intersectionOf>
            </owl:Class>
        </owl:equivalentClass>
        <rdfs:subClassOf rdf:resource="http://www.meteck.org/files/ontologies/stuff.owl#DispersionColloid"/>
        <rdfs:comment xml:lang="en">continuous medium: liquid
dispersed phase: solid
Examples: pigmented ink, blood
http://en.wikipedia.org/wiki/Colloid</rdfs:comment>
    </owl:Class>
    


    <!-- http://www.meteck.org/files/ontologies/stuff.owl#Solid -->

    <owl:Class rdf:about="http://www.meteck.org/files/ontologies/stuff.owl#Solid">
        <rdfs:subClassOf rdf:resource="http://www.meteck.org/files/ontologies/stuff.owl#StuffState"/>
    </owl:Class>
    


    <!-- http://www.meteck.org/files/ontologies/stuff.owl#SolidAerosol -->

    <owl:Class rdf:about="http://www.meteck.org/files/ontologies/stuff.owl#SolidAerosol">
        <owl:equivalentClass>
            <owl:Class>
                <owl:intersectionOf rdf:parseType="Collection">
                    <rdf:Description rdf:about="http://www.meteck.org/files/ontologies/stuff.owl#DispersionColloid"/>
                    <owl:Restriction>
                        <owl:onProperty rdf:resource="http://www.meteck.org/files/ontologies/stuff.owl#hasPartStuff"/>
                        <owl:qualifiedCardinality rdf:datatype="http://www.w3.org/2001/XMLSchema#nonNegativeInteger">1</owl:qualifiedCardinality>
                        <owl:onClass>
                            <owl:Class>
                                <owl:intersectionOf rdf:parseType="Collection">
                                    <rdf:Description rdf:about="http://www.meteck.org/files/ontologies/stuff.owl#Stuff"/>
                                    <owl:Restriction>
                                        <owl:onProperty rdf:resource="http://www.meteck.org/files/ontologies/stuff.owl#hasState"/>
                                        <owl:someValuesFrom rdf:resource="http://www.meteck.org/files/ontologies/stuff.owl#Gas"/>
                                    </owl:Restriction>
                                    <owl:Restriction>
                                        <owl:onProperty>
                                            <rdf:Description>
                                                <owl:inverseOf rdf:resource="http://www.meteck.org/files/ontologies/stuff.owl#srInheresIn"/>
                                            </rdf:Description>
                                        </owl:onProperty>
                                        <owl:someValuesFrom rdf:resource="http://www.meteck.org/files/ontologies/stuff.owl#ContinuousMedium"/>
                                    </owl:Restriction>
                                </owl:intersectionOf>
                            </owl:Class>
                        </owl:onClass>
                    </owl:Restriction>
                    <owl:Restriction>
                        <owl:onProperty rdf:resource="http://www.meteck.org/files/ontologies/stuff.owl#hasPartStuff"/>
                        <owl:qualifiedCardinality rdf:datatype="http://www.w3.org/2001/XMLSchema#nonNegativeInteger">1</owl:qualifiedCardinality>
                        <owl:onClass>
                            <owl:Class>
                                <owl:intersectionOf rdf:parseType="Collection">
                                    <rdf:Description rdf:about="http://www.meteck.org/files/ontologies/stuff.owl#Stuff"/>
                                    <owl:Restriction>
                                        <owl:onProperty rdf:resource="http://www.meteck.org/files/ontologies/stuff.owl#hasState"/>
                                        <owl:someValuesFrom rdf:resource="http://www.meteck.org/files/ontologies/stuff.owl#Solid"/>
                                    </owl:Restriction>
                                    <owl:Restriction>
                                        <owl:onProperty>
                                            <rdf:Description>
                                                <owl:inverseOf rdf:resource="http://www.meteck.org/files/ontologies/stuff.owl#srInheresIn"/>
                                            </rdf:Description>
                                        </owl:onProperty>
                                        <owl:someValuesFrom rdf:resource="http://www.meteck.org/files/ontologies/stuff.owl#DispersedPhase"/>
                                    </owl:Restriction>
                                </owl:intersectionOf>
                            </owl:Class>
                        </owl:onClass>
                    </owl:Restriction>
                </owl:intersectionOf>
            </owl:Class>
        </owl:equivalentClass>
        <rdfs:subClassOf rdf:resource="http://www.meteck.org/files/ontologies/stuff.owl#DispersionColloid"/>
        <rdfs:comment xml:lang="en">continuous medium: gas
dispersed phase: solid
Examples: smoke, cloud, solid particulates
http://en.wikipedia.org/wiki/Colloid</rdfs:comment>
    </owl:Class>
    


    <!-- http://www.meteck.org/files/ontologies/stuff.owl#SolidFoam -->

    <owl:Class rdf:about="http://www.meteck.org/files/ontologies/stuff.owl#SolidFoam">
        <owl:equivalentClass>
            <owl:Class>
                <owl:intersectionOf rdf:parseType="Collection">
                    <rdf:Description rdf:about="http://www.meteck.org/files/ontologies/stuff.owl#DispersionColloid"/>
                    <owl:Restriction>
                        <owl:onProperty rdf:resource="http://www.meteck.org/files/ontologies/stuff.owl#hasPartStuff"/>
                        <owl:qualifiedCardinality rdf:datatype="http://www.w3.org/2001/XMLSchema#nonNegativeInteger">1</owl:qualifiedCardinality>
                        <owl:onClass>
                            <owl:Class>
                                <owl:intersectionOf rdf:parseType="Collection">
                                    <rdf:Description rdf:about="http://www.meteck.org/files/ontologies/stuff.owl#Stuff"/>
                                    <owl:Restriction>
                                        <owl:onProperty rdf:resource="http://www.meteck.org/files/ontologies/stuff.owl#hasState"/>
                                        <owl:someValuesFrom rdf:resource="http://www.meteck.org/files/ontologies/stuff.owl#Gas"/>
                                    </owl:Restriction>
                                    <owl:Restriction>
                                        <owl:onProperty>
                                            <rdf:Description>
                                                <owl:inverseOf rdf:resource="http://www.meteck.org/files/ontologies/stuff.owl#srInheresIn"/>
                                            </rdf:Description>
                                        </owl:onProperty>
                                        <owl:someValuesFrom rdf:resource="http://www.meteck.org/files/ontologies/stuff.owl#DispersedPhase"/>
                                    </owl:Restriction>
                                </owl:intersectionOf>
                            </owl:Class>
                        </owl:onClass>
                    </owl:Restriction>
                    <owl:Restriction>
                        <owl:onProperty rdf:resource="http://www.meteck.org/files/ontologies/stuff.owl#hasPartStuff"/>
                        <owl:qualifiedCardinality rdf:datatype="http://www.w3.org/2001/XMLSchema#nonNegativeInteger">1</owl:qualifiedCardinality>
                        <owl:onClass>
                            <owl:Class>
                                <owl:intersectionOf rdf:parseType="Collection">
                                    <rdf:Description rdf:about="http://www.meteck.org/files/ontologies/stuff.owl#Stuff"/>
                                    <owl:Restriction>
                                        <owl:onProperty rdf:resource="http://www.meteck.org/files/ontologies/stuff.owl#hasState"/>
                                        <owl:someValuesFrom rdf:resource="http://www.meteck.org/files/ontologies/stuff.owl#Solid"/>
                                    </owl:Restriction>
                                    <owl:Restriction>
                                        <owl:onProperty>
                                            <rdf:Description>
                                                <owl:inverseOf rdf:resource="http://www.meteck.org/files/ontologies/stuff.owl#srInheresIn"/>
                                            </rdf:Description>
                                        </owl:onProperty>
                                        <owl:someValuesFrom rdf:resource="http://www.meteck.org/files/ontologies/stuff.owl#ContinuousMedium"/>
                                    </owl:Restriction>
                                </owl:intersectionOf>
                            </owl:Class>
                        </owl:onClass>
                    </owl:Restriction>
                </owl:intersectionOf>
            </owl:Class>
        </owl:equivalentClass>
        <rdfs:subClassOf rdf:resource="http://www.meteck.org/files/ontologies/stuff.owl#DispersionColloid"/>
        <rdfs:comment xml:lang="en">continuous medium: solid
dispersed phase: gas
Examples: aerogel, styrofoam
http://en.wikipedia.org/wiki/Colloid</rdfs:comment>
    </owl:Class>
    


    <!-- http://www.meteck.org/files/ontologies/stuff.owl#SolidHeterogeneousMixture -->

    <owl:Class rdf:about="http://www.meteck.org/files/ontologies/stuff.owl#SolidHeterogeneousMixture">
        <owl:equivalentClass>
            <owl:Class>
                <owl:intersectionOf rdf:parseType="Collection">
                    <rdf:Description rdf:about="http://www.meteck.org/files/ontologies/stuff.owl#HeterogeneousMixture"/>
                    <owl:Restriction>
                        <owl:onProperty rdf:resource="http://www.meteck.org/files/ontologies/stuff.owl#hasPartStuff"/>
                        <owl:minQualifiedCardinality rdf:datatype="http://www.w3.org/2001/XMLSchema#nonNegativeInteger">2</owl:minQualifiedCardinality>
                        <owl:onClass>
                            <owl:Class>
                                <owl:intersectionOf rdf:parseType="Collection">
                                    <rdf:Description rdf:about="http://www.meteck.org/files/ontologies/stuff.owl#Stuff"/>
                                    <owl:Restriction>
                                        <owl:onProperty rdf:resource="http://www.meteck.org/files/ontologies/stuff.owl#hasState"/>
                                        <owl:someValuesFrom rdf:resource="http://www.meteck.org/files/ontologies/stuff.owl#Solid"/>
                                    </owl:Restriction>
                                </owl:intersectionOf>
                            </owl:Class>
                        </owl:onClass>
                    </owl:Restriction>
                </owl:intersectionOf>
            </owl:Class>
        </owl:equivalentClass>
        <rdfs:subClassOf rdf:resource="http://www.meteck.org/files/ontologies/stuff.owl#HeterogeneousMixture"/>
        <rdfs:comment xml:lang="en">the solid version of a suspension (heterogenous mixture, not homogenised).
Example: wood has a compartmentalisation of the components (cellulose, hemicellulose, ligning, and other stuffs called &apos;extractives&apos; [plant hormone, waxes, terpenes, etc.]).</rdfs:comment>
    </owl:Class>
    


    <!-- http://www.meteck.org/files/ontologies/stuff.owl#SolidSol -->

    <owl:Class rdf:about="http://www.meteck.org/files/ontologies/stuff.owl#SolidSol">
        <owl:equivalentClass>
            <owl:Class>
                <owl:intersectionOf rdf:parseType="Collection">
                    <rdf:Description rdf:about="http://www.meteck.org/files/ontologies/stuff.owl#DispersionColloid"/>
                    <owl:Restriction>
                        <owl:onProperty rdf:resource="http://www.meteck.org/files/ontologies/stuff.owl#hasPartStuff"/>
                        <owl:qualifiedCardinality rdf:datatype="http://www.w3.org/2001/XMLSchema#nonNegativeInteger">1</owl:qualifiedCardinality>
                        <owl:onClass>
                            <owl:Class>
                                <owl:intersectionOf rdf:parseType="Collection">
                                    <rdf:Description rdf:about="http://www.meteck.org/files/ontologies/stuff.owl#Stuff"/>
                                    <owl:Restriction>
                                        <owl:onProperty rdf:resource="http://www.meteck.org/files/ontologies/stuff.owl#hasState"/>
                                        <owl:someValuesFrom rdf:resource="http://www.meteck.org/files/ontologies/stuff.owl#Solid"/>
                                    </owl:Restriction>
                                    <owl:Restriction>
                                        <owl:onProperty>
                                            <rdf:Description>
                                                <owl:inverseOf rdf:resource="http://www.meteck.org/files/ontologies/stuff.owl#srInheresIn"/>
                                            </rdf:Description>
                                        </owl:onProperty>
                                        <owl:someValuesFrom rdf:resource="http://www.meteck.org/files/ontologies/stuff.owl#ContinuousMedium"/>
                                    </owl:Restriction>
                                </owl:intersectionOf>
                            </owl:Class>
                        </owl:onClass>
                    </owl:Restriction>
                    <owl:Restriction>
                        <owl:onProperty rdf:resource="http://www.meteck.org/files/ontologies/stuff.owl#hasPartStuff"/>
                        <owl:qualifiedCardinality rdf:datatype="http://www.w3.org/2001/XMLSchema#nonNegativeInteger">1</owl:qualifiedCardinality>
                        <owl:onClass>
                            <owl:Class>
                                <owl:intersectionOf rdf:parseType="Collection">
                                    <rdf:Description rdf:about="http://www.meteck.org/files/ontologies/stuff.owl#Stuff"/>
                                    <owl:Restriction>
                                        <owl:onProperty rdf:resource="http://www.meteck.org/files/ontologies/stuff.owl#hasState"/>
                                        <owl:someValuesFrom rdf:resource="http://www.meteck.org/files/ontologies/stuff.owl#Solid"/>
                                    </owl:Restriction>
                                    <owl:Restriction>
                                        <owl:onProperty>
                                            <rdf:Description>
                                                <owl:inverseOf rdf:resource="http://www.meteck.org/files/ontologies/stuff.owl#srInheresIn"/>
                                            </rdf:Description>
                                        </owl:onProperty>
                                        <owl:someValuesFrom rdf:resource="http://www.meteck.org/files/ontologies/stuff.owl#DispersedPhase"/>
                                    </owl:Restriction>
                                </owl:intersectionOf>
                            </owl:Class>
                        </owl:onClass>
                    </owl:Restriction>
                </owl:intersectionOf>
            </owl:Class>
        </owl:equivalentClass>
        <rdfs:subClassOf rdf:resource="http://www.meteck.org/files/ontologies/stuff.owl#DispersionColloid"/>
        <rdfs:comment xml:lang="en">continuous medium: solid
dispersed phase: solid
Examples: cranberry glass
http://en.wikipedia.org/wiki/Colloid</rdfs:comment>
    </owl:Class>
    


    <!-- http://www.meteck.org/files/ontologies/stuff.owl#Solute -->

    <owl:Class rdf:about="http://www.meteck.org/files/ontologies/stuff.owl#Solute">
        <rdfs:subClassOf rdf:resource="http://www.meteck.org/files/ontologies/stuff.owl#StuffRole"/>
        <rdfs:subClassOf>
            <owl:Restriction>
                <owl:onProperty>
                    <rdf:Description>
                        <owl:inverseOf rdf:resource="http://www.meteck.org/files/ontologies/stuff.owl#solutionFormingRelation"/>
                    </rdf:Description>
                </owl:onProperty>
                <owl:someValuesFrom rdf:resource="http://www.meteck.org/files/ontologies/stuff.owl#Solvent"/>
            </owl:Restriction>
        </rdfs:subClassOf>
        <owl:disjointWith rdf:resource="http://www.meteck.org/files/ontologies/stuff.owl#Solvent"/>
        <rdfs:comment>A substance dissolved in another substance (the solvent)</rdfs:comment>
    </owl:Class>
    


    <!-- http://www.meteck.org/files/ontologies/stuff.owl#Solution -->

    <owl:Class rdf:about="http://www.meteck.org/files/ontologies/stuff.owl#Solution">
        <owl:equivalentClass>
            <owl:Class>
                <owl:intersectionOf rdf:parseType="Collection">
                    <rdf:Description rdf:about="http://www.meteck.org/files/ontologies/stuff.owl#HomogeneousMixture"/>
                    <owl:Restriction>
                        <owl:onProperty rdf:resource="http://www.meteck.org/files/ontologies/stuff.owl#hasPartStuff"/>
                        <owl:someValuesFrom>
                            <owl:Class>
                                <owl:intersectionOf rdf:parseType="Collection">
                                    <rdf:Description rdf:about="http://www.meteck.org/files/ontologies/stuff.owl#Stuff"/>
                                    <owl:Restriction>
                                        <owl:onProperty>
                                            <rdf:Description>
                                                <owl:inverseOf rdf:resource="http://www.meteck.org/files/ontologies/stuff.owl#srInheresIn"/>
                                            </rdf:Description>
                                        </owl:onProperty>
                                        <owl:someValuesFrom rdf:resource="http://www.meteck.org/files/ontologies/stuff.owl#Solute"/>
                                    </owl:Restriction>
                                    <owl:Restriction>
                                        <owl:onProperty rdf:resource="http://www.meteck.org/files/ontologies/stuff.owl#hasGranuleType"/>
                                        <owl:allValuesFrom>
                                            <owl:Class>
                                                <owl:unionOf rdf:parseType="Collection">
                                                    <rdf:Description rdf:about="http://www.meteck.org/files/ontologies/stuff.owl#Atom"/>
                                                    <rdf:Description rdf:about="http://www.meteck.org/files/ontologies/stuff.owl#Ion"/>
                                                    <rdf:Description rdf:about="http://www.meteck.org/files/ontologies/stuff.owl#Molecule"/>
                                                </owl:unionOf>
                                            </owl:Class>
                                        </owl:allValuesFrom>
                                    </owl:Restriction>
                                </owl:intersectionOf>
                            </owl:Class>
                        </owl:someValuesFrom>
                    </owl:Restriction>
                    <owl:Restriction>
                        <owl:onProperty rdf:resource="http://www.meteck.org/files/ontologies/stuff.owl#hasPartStuff"/>
                        <owl:someValuesFrom>
                            <owl:Class>
                                <owl:intersectionOf rdf:parseType="Collection">
                                    <rdf:Description rdf:about="http://www.meteck.org/files/ontologies/stuff.owl#Stuff"/>
                                    <owl:Restriction>
                                        <owl:onProperty>
                                            <rdf:Description>
                                                <owl:inverseOf rdf:resource="http://www.meteck.org/files/ontologies/stuff.owl#srInheresIn"/>
                                            </rdf:Description>
                                        </owl:onProperty>
                                        <owl:someValuesFrom rdf:resource="http://www.meteck.org/files/ontologies/stuff.owl#Solvent"/>
                                    </owl:Restriction>
                                    <owl:Restriction>
                                        <owl:onProperty rdf:resource="http://www.meteck.org/files/ontologies/stuff.owl#hasGranuleType"/>
                                        <owl:allValuesFrom>
                                            <owl:Class>
                                                <owl:unionOf rdf:parseType="Collection">
                                                    <rdf:Description rdf:about="http://www.meteck.org/files/ontologies/stuff.owl#Atom"/>
                                                    <rdf:Description rdf:about="http://www.meteck.org/files/ontologies/stuff.owl#Ion"/>
                                                    <rdf:Description rdf:about="http://www.meteck.org/files/ontologies/stuff.owl#Molecule"/>
                                                </owl:unionOf>
                                            </owl:Class>
                                        </owl:allValuesFrom>
                                    </owl:Restriction>
                                </owl:intersectionOf>
                            </owl:Class>
                        </owl:someValuesFrom>
                    </owl:Restriction>
                    <owl:Restriction>
                        <owl:onProperty rdf:resource="http://www.meteck.org/files/ontologies/stuff.owl#hasNrOfPhase"/>
                        <owl:someValuesFrom>
                            <rdfs:Datatype>
                                <owl:onDatatype rdf:resource="http://www.w3.org/2001/XMLSchema#int"/>
                                <owl:withRestrictions rdf:parseType="Collection">
                                    <rdf:Description>
                                        <xsd:maxInclusive rdf:datatype="http://www.w3.org/2001/XMLSchema#integer">1</xsd:maxInclusive>
                                    </rdf:Description>
                                </owl:withRestrictions>
                            </rdfs:Datatype>
                        </owl:someValuesFrom>
                    </owl:Restriction>
                </owl:intersectionOf>
            </owl:Class>
        </owl:equivalentClass>
        <rdfs:subClassOf rdf:resource="http://www.meteck.org/files/ontologies/stuff.owl#HomogeneousMixture"/>
        <rdfs:comment xml:lang="en">Combination of at least two stuffs where the mixing occurs at the molecular level (i.e., involves some chemical reaction), and therewith may form a new substance (a compound). a solution&apos;s composition is uniform. note that solutions can exist in all three physical states (i.e., not just in the liquid state, as it is used in the vernacular).
We ignore here the &apos;dilute solution&apos; [http://goldbook.iupac.org/D01739.html] which has a non-crisp cut-off point (&quot;sum of amount fractions of all the solutes is small compared to 1&quot;, according to the GoldBook)</rdfs:comment>
        <rdfs:comment>the &quot;and hasNrOfPhase some integer[&gt; &quot;0&quot;^^integer]&quot; and &quot;and hasNrOfPhase some integer[=&lt; &quot;1&quot;^^integer]&quot; is because the interface didn&apos;t accept =1</rdfs:comment>
    </owl:Class>
    


    <!-- http://www.meteck.org/files/ontologies/stuff.owl#Solvent -->

    <owl:Class rdf:about="http://www.meteck.org/files/ontologies/stuff.owl#Solvent">
        <rdfs:subClassOf rdf:resource="http://www.meteck.org/files/ontologies/stuff.owl#StuffRole"/>
        <rdfs:comment>A substance in which another substance (the solute) is dissolved</rdfs:comment>
        <rdfs:comment>The solutionFormingRelation is a bit of a catch-all for the chemical reactions that occur when te solute is dissolved in the solvent</rdfs:comment>
    </owl:Class>
    


    <!-- http://www.meteck.org/files/ontologies/stuff.owl#State -->

    <owl:Class rdf:about="http://www.meteck.org/files/ontologies/stuff.owl#State">
        <rdfs:subClassOf rdf:resource="http://www.meteck.org/files/ontologies/stuff.owl#Perdurant"/>
    </owl:Class>
    


    <!-- http://www.meteck.org/files/ontologies/stuff.owl#StructuredPureStuff -->

    <owl:Class rdf:about="http://www.meteck.org/files/ontologies/stuff.owl#StructuredPureStuff">
        <owl:equivalentClass>
            <owl:Class>
                <owl:intersectionOf rdf:parseType="Collection">
                    <rdf:Description rdf:about="http://www.meteck.org/files/ontologies/stuff.owl#PureStuff"/>
                    <owl:Restriction>
                        <owl:onProperty rdf:resource="http://www.meteck.org/files/ontologies/stuff.owl#hasGranuleType"/>
                        <owl:allValuesFrom rdf:resource="http://www.meteck.org/files/ontologies/stuff.owl#Molecule"/>
                    </owl:Restriction>
                    <owl:Restriction>
                        <owl:onProperty rdf:resource="http://www.meteck.org/files/ontologies/stuff.owl#hasGranuleType"/>
                        <owl:qualifiedCardinality rdf:datatype="http://www.w3.org/2001/XMLSchema#nonNegativeInteger">1</owl:qualifiedCardinality>
                        <owl:onClass rdf:resource="http://www.meteck.org/files/ontologies/stuff.owl#Molecule"/>
                    </owl:Restriction>
                </owl:intersectionOf>
            </owl:Class>
        </owl:equivalentClass>
        <rdfs:subClassOf rdf:resource="http://www.meteck.org/files/ontologies/stuff.owl#PureStuff"/>
        <owl:disjointWith rdf:resource="http://www.meteck.org/files/ontologies/stuff.owl#UnstructuredPureStuff"/>
        <rdfs:comment xml:lang="en">Stuff that consists of the same kind of molecules (give or take the finer-grained conformation changes, temporary dissociations of, say, H, the occasional D in the &apos;H2O&apos; etc.).
Examples: an amount of water (H2O), an amount of tablesugar (glucose-fructose), silica/silicon dioxide (SiO2), vitamin A, etc.</rdfs:comment>
        <rdfs:comment>synonym: Compound</rdfs:comment>
        <rdfs:comment xml:lang="en">there should be a &apos;has basis type exactly *one type of* molecule&apos; (ok, we ignore the minor impurities here), not just one single individual molecule.</rdfs:comment>
    </owl:Class>
    


    <!-- http://www.meteck.org/files/ontologies/stuff.owl#Stuff -->

    <owl:Class rdf:about="http://www.meteck.org/files/ontologies/stuff.owl#Stuff">
        <rdfs:subClassOf rdf:resource="http://www.meteck.org/files/ontologies/stuff.owl#PhysicalEndurant"/>
        <rdfs:subClassOf>
            <owl:Restriction>
                <owl:onProperty rdf:resource="http://www.meteck.org/files/ontologies/stuff.owl#hasState"/>
                <owl:allValuesFrom rdf:resource="http://www.meteck.org/files/ontologies/stuff.owl#StuffState"/>
            </owl:Restriction>
        </rdfs:subClassOf>
        <rdfs:subClassOf>
            <owl:Restriction>
                <owl:onProperty rdf:resource="http://www.meteck.org/files/ontologies/stuff.owl#hasState"/>
                <owl:maxQualifiedCardinality rdf:datatype="http://www.w3.org/2001/XMLSchema#nonNegativeInteger">3</owl:maxQualifiedCardinality>
                <owl:onClass rdf:resource="http://www.meteck.org/files/ontologies/stuff.owl#StuffState"/>
            </owl:Restriction>
        </rdfs:subClassOf>
        <owl:disjointUnionOf rdf:parseType="Collection">
            <rdf:Description rdf:about="http://www.meteck.org/files/ontologies/stuff.owl#MixedStuff"/>
            <rdf:Description rdf:about="http://www.meteck.org/files/ontologies/stuff.owl#PureStuff"/>
        </owl:disjointUnionOf>
        <rdfs:comment xml:lang="en">Synonym: Amount of Matter</rdfs:comment>
    </owl:Class>
    


    <!-- http://www.meteck.org/files/ontologies/stuff.owl#StuffRole -->

    <owl:Class rdf:about="http://www.meteck.org/files/ontologies/stuff.owl#StuffRole">
        <rdfs:subClassOf rdf:resource="http://www.meteck.org/files/ontologies/stuff.owl#Role"/>
        <rdfs:subClassOf>
            <owl:Restriction>
                <owl:onProperty rdf:resource="http://www.meteck.org/files/ontologies/stuff.owl#srInheresIn"/>
                <owl:someValuesFrom rdf:resource="http://www.meteck.org/files/ontologies/stuff.owl#Stuff"/>
            </owl:Restriction>
        </rdfs:subClassOf>
        <rdfs:comment>The role a stuff plays in a mixture.</rdfs:comment>
    </owl:Class>
    


    <!-- http://www.meteck.org/files/ontologies/stuff.owl#StuffState -->

    <owl:Class rdf:about="http://www.meteck.org/files/ontologies/stuff.owl#StuffState">
        <rdfs:subClassOf rdf:resource="http://www.meteck.org/files/ontologies/stuff.owl#State"/>
        <rdfs:comment xml:lang="en">This should be refined. 
On the one hand, we can have, say, water in the solid state, in the liquid state and in the gaseous state. 
On the other hand, when considering colloids, then one of the two stuffs is in one state and the other either in the same state or in another state, regardless the actual stuff type (like whether it is liquid sunflower oil or lineseed oil, or CO2 gas or air). That is, for colloids, the state the stuff is in when mixing is the defining characteristics. Here, with the stuffs, we are interested in the state in general, not the state of a stuff.</rdfs:comment>
    </owl:Class>
    


    <!-- http://www.meteck.org/files/ontologies/stuff.owl#Suspension -->

    <owl:Class rdf:about="http://www.meteck.org/files/ontologies/stuff.owl#Suspension">
        <owl:equivalentClass>
            <owl:Class>
                <owl:intersectionOf rdf:parseType="Collection">
                    <rdf:Description rdf:about="http://www.meteck.org/files/ontologies/stuff.owl#HeterogeneousMixture"/>
                    <owl:Restriction>
                        <owl:onProperty rdf:resource="http://www.meteck.org/files/ontologies/stuff.owl#hasPartStuff"/>
                        <owl:someValuesFrom>
                            <owl:Class>
                                <owl:intersectionOf rdf:parseType="Collection">
                                    <rdf:Description rdf:about="http://www.meteck.org/files/ontologies/stuff.owl#Stuff"/>
                                    <owl:Restriction>
                                        <owl:onProperty rdf:resource="http://www.meteck.org/files/ontologies/stuff.owl#hasState"/>
                                        <owl:someValuesFrom rdf:resource="http://www.meteck.org/files/ontologies/stuff.owl#Liquid"/>
                                    </owl:Restriction>
                                    <owl:Restriction>
                                        <owl:onProperty>
                                            <rdf:Description>
                                                <owl:inverseOf rdf:resource="http://www.meteck.org/files/ontologies/stuff.owl#srInheresIn"/>
                                            </rdf:Description>
                                        </owl:onProperty>
                                        <owl:someValuesFrom rdf:resource="http://www.meteck.org/files/ontologies/stuff.owl#ContinuousMedium"/>
                                    </owl:Restriction>
                                </owl:intersectionOf>
                            </owl:Class>
                        </owl:someValuesFrom>
                    </owl:Restriction>
                    <owl:Restriction>
                        <owl:onProperty rdf:resource="http://www.meteck.org/files/ontologies/stuff.owl#hasPartStuff"/>
                        <owl:someValuesFrom>
                            <owl:Class>
                                <owl:intersectionOf rdf:parseType="Collection">
                                    <rdf:Description rdf:about="http://www.meteck.org/files/ontologies/stuff.owl#Stuff"/>
                                    <owl:Restriction>
                                        <owl:onProperty rdf:resource="http://www.meteck.org/files/ontologies/stuff.owl#hasState"/>
                                        <owl:someValuesFrom rdf:resource="http://www.meteck.org/files/ontologies/stuff.owl#Solid"/>
                                    </owl:Restriction>
                                    <owl:Restriction>
                                        <owl:onProperty>
                                            <rdf:Description>
                                                <owl:inverseOf rdf:resource="http://www.meteck.org/files/ontologies/stuff.owl#srInheresIn"/>
                                            </rdf:Description>
                                        </owl:onProperty>
                                        <owl:someValuesFrom rdf:resource="http://www.meteck.org/files/ontologies/stuff.owl#DispersedPhase"/>
                                    </owl:Restriction>
                                </owl:intersectionOf>
                            </owl:Class>
                        </owl:someValuesFrom>
                    </owl:Restriction>
                </owl:intersectionOf>
            </owl:Class>
        </owl:equivalentClass>
        <rdfs:subClassOf rdf:resource="http://www.meteck.org/files/ontologies/stuff.owl#HeterogeneousMixture"/>
        <rdfs:subClassOf>
            <owl:Class>
                <owl:intersectionOf rdf:parseType="Collection">
                    <owl:Restriction>
                        <owl:onProperty rdf:resource="http://www.meteck.org/files/ontologies/stuff.owl#hasGranuleType"/>
                        <owl:someValuesFrom rdf:resource="http://www.meteck.org/files/ontologies/stuff.owl#Molecule"/>
                    </owl:Restriction>
                    <owl:Restriction>
                        <owl:onProperty rdf:resource="http://www.meteck.org/files/ontologies/stuff.owl#hasGranuleType"/>
                        <owl:someValuesFrom rdf:resource="http://www.meteck.org/files/ontologies/stuff.owl#MultiMoleculeParticle"/>
                    </owl:Restriction>
                </owl:intersectionOf>
            </owl:Class>
        </rdfs:subClassOf>
        <rdfs:comment xml:lang="en">heterogenous mixture of larger particles in a liquid, and that substance naturally separates (i.e., separation due to sedimentation, creaming, flocculation, or coalescence, unless &apos;stabilized&apos; and &apos;homogenised&apos; [as regularly happens in the production process]). E.g. tomato juice, mud.
TBA: the particle size of the solid is usually &gt;1 micron</rdfs:comment>
    </owl:Class>
    


    <!-- http://www.meteck.org/files/ontologies/stuff.owl#UnevenDistribution -->

    <owl:Class rdf:about="http://www.meteck.org/files/ontologies/stuff.owl#UnevenDistribution">
        <rdfs:subClassOf rdf:resource="http://www.meteck.org/files/ontologies/stuff.owl#AbstractRegion"/>
    </owl:Class>
    


    <!-- http://www.meteck.org/files/ontologies/stuff.owl#UnstructuredPureStuff -->

    <owl:Class rdf:about="http://www.meteck.org/files/ontologies/stuff.owl#UnstructuredPureStuff">
        <owl:equivalentClass>
            <owl:Class>
                <owl:intersectionOf rdf:parseType="Collection">
                    <rdf:Description rdf:about="http://www.meteck.org/files/ontologies/stuff.owl#PureStuff"/>
                    <owl:Restriction>
                        <owl:onProperty rdf:resource="http://www.meteck.org/files/ontologies/stuff.owl#hasGranuleType"/>
                        <owl:allValuesFrom rdf:resource="http://www.meteck.org/files/ontologies/stuff.owl#Atom"/>
                    </owl:Restriction>
                    <owl:Restriction>
                        <owl:onProperty rdf:resource="http://www.meteck.org/files/ontologies/stuff.owl#hasGranuleType"/>
                        <owl:qualifiedCardinality rdf:datatype="http://www.w3.org/2001/XMLSchema#nonNegativeInteger">1</owl:qualifiedCardinality>
                        <owl:onClass rdf:resource="http://www.meteck.org/files/ontologies/stuff.owl#Atom"/>
                    </owl:Restriction>
                </owl:intersectionOf>
            </owl:Class>
        </owl:equivalentClass>
        <rdfs:subClassOf rdf:resource="http://www.meteck.org/files/ontologies/stuff.owl#PureStuff"/>
        <rdfs:comment xml:lang="en">Stuff that consists of the same kind of atoms.
Examples: an amount of helium, an amount of gold
Realistically, there may well be undetectable impurities, and so on, but we don&apos;t care about that here</rdfs:comment>
        <rdfs:comment>synonym: Element</rdfs:comment>
        <rdfs:comment xml:lang="en">this definition is actually meant as &apos;has basis type exactly *one type of* atom&apos;, not just one single individual atom.</rdfs:comment>
    </owl:Class>
    


    <!-- http://www.wurvoc.org/vocabularies/om-1.8/Phenomenon -->

    <rdf:Description rdf:about="http://www.wurvoc.org/vocabularies/om-1.8/Phenomenon"/>
    


    <!-- http://www.wurvoc.org/vocabularies/om-1.8/Quantity -->

    <rdf:Description rdf:about="http://www.wurvoc.org/vocabularies/om-1.8/Quantity">
        <rdfs:subClassOf rdf:resource="http://www.meteck.org/files/ontologies/stuff.owl#Region"/>
    </rdf:Description>
    


    <!-- http://www.wurvoc.org/vocabularies/om-1.8/Unit_of_measure -->

    <rdf:Description rdf:about="http://www.wurvoc.org/vocabularies/om-1.8/Unit_of_measure">
        <rdfs:subClassOf rdf:resource="http://www.meteck.org/files/ontologies/stuff.owl#Abstract"/>
    </rdf:Description>
    <rdf:Description>
        <owl:qualifiedCardinality rdf:datatype="http://www.w3.org/2001/XMLSchema#nonNegativeInteger">1</owl:qualifiedCardinality>
    </rdf:Description>
    


    <!-- 
    ///////////////////////////////////////////////////////////////////////////////////////
    //
    // General axioms
    //
    ///////////////////////////////////////////////////////////////////////////////////////
     -->

    <rdf:Description>
        <rdf:type rdf:resource="http://www.w3.org/2002/07/owl#AllDisjointClasses"/>
        <owl:members rdf:parseType="Collection">
            <rdf:Description rdf:about="http://www.meteck.org/files/ontologies/stuff.owl#Abstract"/>
            <rdf:Description rdf:about="http://www.meteck.org/files/ontologies/stuff.owl#Endurant"/>
            <rdf:Description rdf:about="http://www.meteck.org/files/ontologies/stuff.owl#Perdurant"/>
            <rdf:Description rdf:about="http://www.meteck.org/files/ontologies/stuff.owl#Quality"/>
        </owl:members>
    </rdf:Description>
    <rdf:Description>
        <rdf:type rdf:resource="http://www.w3.org/2002/07/owl#AllDisjointClasses"/>
        <owl:members rdf:parseType="Collection">
            <rdf:Description rdf:about="http://www.meteck.org/files/ontologies/stuff.owl#AmountOfStuff"/>
            <rdf:Description rdf:about="http://www.meteck.org/files/ontologies/stuff.owl#Atom"/>
            <rdf:Description rdf:about="http://www.meteck.org/files/ontologies/stuff.owl#Ion"/>
            <rdf:Description rdf:about="http://www.meteck.org/files/ontologies/stuff.owl#Molecule"/>
            <rdf:Description rdf:about="http://www.meteck.org/files/ontologies/stuff.owl#MultiMoleculeParticle"/>
        </owl:members>
    </rdf:Description>
    <rdf:Description>
        <rdf:type rdf:resource="http://www.w3.org/2002/07/owl#AllDisjointClasses"/>
        <owl:members rdf:parseType="Collection">
            <rdf:Description rdf:about="http://www.meteck.org/files/ontologies/stuff.owl#AssociationalColloid"/>
            <rdf:Description rdf:about="http://www.meteck.org/files/ontologies/stuff.owl#DispersionColloid"/>
            <rdf:Description rdf:about="http://www.meteck.org/files/ontologies/stuff.owl#MolecularColloid"/>
        </owl:members>
    </rdf:Description>
    <rdf:Description>
        <rdf:type rdf:resource="http://www.w3.org/2002/07/owl#AllDisjointClasses"/>
        <owl:members rdf:parseType="Collection">
            <rdf:Description rdf:about="http://www.meteck.org/files/ontologies/stuff.owl#Atom"/>
            <rdf:Description rdf:about="http://www.meteck.org/files/ontologies/stuff.owl#Ion"/>
            <rdf:Description rdf:about="http://www.meteck.org/files/ontologies/stuff.owl#Molecule"/>
            <rdf:Description rdf:about="http://www.meteck.org/files/ontologies/stuff.owl#MultiMoleculeParticle"/>
        </owl:members>
    </rdf:Description>
    <rdf:Description>
        <rdf:type rdf:resource="http://www.w3.org/2002/07/owl#AllDisjointClasses"/>
        <owl:members rdf:parseType="Collection">
            <rdf:Description rdf:about="http://www.meteck.org/files/ontologies/stuff.owl#Emulsion"/>
            <rdf:Description rdf:about="http://www.meteck.org/files/ontologies/stuff.owl#Foam"/>
            <rdf:Description rdf:about="http://www.meteck.org/files/ontologies/stuff.owl#Gel"/>
            <rdf:Description rdf:about="http://www.meteck.org/files/ontologies/stuff.owl#LiquidAerosol"/>
            <rdf:Description rdf:about="http://www.meteck.org/files/ontologies/stuff.owl#Sol"/>
            <rdf:Description rdf:about="http://www.meteck.org/files/ontologies/stuff.owl#SolidAerosol"/>
            <rdf:Description rdf:about="http://www.meteck.org/files/ontologies/stuff.owl#SolidFoam"/>
            <rdf:Description rdf:about="http://www.meteck.org/files/ontologies/stuff.owl#SolidSol"/>
        </owl:members>
    </rdf:Description>
    <rdf:Description>
        <rdf:type rdf:resource="http://www.w3.org/2002/07/owl#AllDisjointClasses"/>
        <owl:members rdf:parseType="Collection">
            <rdf:Description rdf:about="http://www.meteck.org/files/ontologies/stuff.owl#Gas"/>
            <rdf:Description rdf:about="http://www.meteck.org/files/ontologies/stuff.owl#Liquid"/>
            <rdf:Description rdf:about="http://www.meteck.org/files/ontologies/stuff.owl#Solid"/>
        </owl:members>
    </rdf:Description>
</rdf:RDF>



<!-- Generated by the OWL API (version 4.2.8.20170104-2310) https://github.com/owlcs/owlapi -->

