<?xml version="1.0"?>
<rdf:RDF xmlns="https://w3id.org/polifonia/ontology/music-instrument/"
     xml:base="https://w3id.org/polifonia/ontology/music-instrument/"
     xmlns:dc="http://purl.org/dc/elements/1.1/"
     xmlns:owl="http://www.w3.org/2002/07/owl#"
     xmlns:rdf="http://www.w3.org/1999/02/22-rdf-syntax-ns#"
     xmlns:xml="http://www.w3.org/XML/1998/namespace"
     xmlns:xsd="http://www.w3.org/2001/XMLSchema#"
     xmlns:core="https://w3id.org/polifonia/ontology/core/"
     xmlns:inst="https://w3id.org/polifonia/ontology/music-instrument/"
     xmlns:opla="http://ontologydesignpatterns.org/opla/"
     xmlns:rdfs="http://www.w3.org/2000/01/rdf-schema#"
     xmlns:terms="http://purl.org/dc/terms/"
     xmlns:cc="http://creativecommons.org/ns#"
     xmlns:vann="http://purl.org/vocab/vann/"
     xmlns:catalogue="https://w3id.org/arco/ontology/catalogue/">
    <owl:Ontology rdf:about="https://w3id.org/polifonia/ontology/music-instrument/">
        <owl:versionIRI rdf:resource="https://w3id.org/polifonia/ontology/music-instrument/1.0/"/>
        <owl:imports rdf:resource="https://w3id.org/arco/ontology/location/1.2"/>
        <owl:imports rdf:resource="https://w3id.org/polifonia/ontology/core/1.0"/>
        <owl:imports rdf:resource="https://w3id.org/polifonia/ontology/music-meta/1.0/"/>
        <dc:creator xml:lang="en">Jacopo de Berardinis</dc:creator>
        <dc:creator xml:lang="en">Valentina Carriero</dc:creator>
        <dc:creator xml:lang="en">Valentina Presutti</dc:creator>
        <dc:license rdf:resource="https://creativecommons.org/licenses/by-sa/4.0/"/>
        <terms:license rdf:resource="https://creativecommons.org/licenses/by-sa/4.0/"/>
        <cc:license rdf:resource="https://creativecommons.org/licenses/by-sa/4.0/"/>
        <rdfs:comment xml:lang="en">This ontology describes musical instruments as mediums of performance and their technical properties. Given that numerous taxonomies of instruments into groups and families exist (e.g. Hornbostel-Sachs, MIMO, MusicBrainz) and finding common categorisations is an open problem, our module provides an abstraction capable to express arbitrary classifications.</rdfs:comment>
        <rdfs:label xml:lang="en">Music Instrument Ontology</rdfs:label>
        <dc:title xml:lang="en">Music Instrument Ontology</dc:title>
        <dc:description xml:lang="en">This ontology describes musical instruments as mediums of performance and their technical properties. Given that numerous taxonomies of instruments into groups and families exist (e.g. Hornbostel-Sachs, MIMO, MusicBrainz) and finding common categorisations is an open problem, our module provides an abstraction capable to express arbitrary classifications.</dc:description>
        <owl:versionInfo xml:lang="en">1.0</owl:versionInfo>
        <terms:modified>"2023-05-19"^^xsd:date</terms:modified>
        <terms:issued>"2023-04-12"^^xsd:date</terms:issued>
        <vann:preferredNamespacePrefix>mi:</vann:preferredNamespacePrefix>
        <vann:preferredNamespaceUri>https://w3id.org/polifonia/ontology/music-instrument/</vann:preferredNamespaceUri>
    </owl:Ontology>
    


    <!-- 
    ///////////////////////////////////////////////////////////////////////////////////////
    //
    // Object Properties
    //
    ///////////////////////////////////////////////////////////////////////////////////////
     -->

    


    <!-- https://w3id.org/polifonia/ontology/instrument/hasBuilder -->

    <owl:ObjectProperty rdf:about="https://w3id.org/polifonia/ontology/instrument/hasBuilder">
        <rdfs:domain rdf:resource="https://w3id.org/polifonia/ontology/instrument/InstrumentRealization"/>
        <rdfs:range rdf:resource="https://w3id.org/polifonia/ontology/core/Agent"/>
        <rdfs:comment xml:lang="en">The relation between an instrument realization and its builder.</rdfs:comment>
        <rdfs:label xml:lang="en">has builder</rdfs:label>
    </owl:ObjectProperty>
    


    <!-- https://w3id.org/polifonia/ontology/instrument/wasBuiltAtTime -->

    <owl:ObjectProperty rdf:about="https://w3id.org/polifonia/ontology/instrument/wasBuiltAtTime">
        <rdfs:domain rdf:resource="https://w3id.org/polifonia/ontology/instrument/InstrumentRealization"/>
        <rdfs:range rdf:resource="https://w3id.org/polifonia/ontology/core/TimeInterval"/>
        <rdfs:comment xml:lang="en">The relation between an instrument realization and the time interval it was built at.</rdfs:comment>
        <rdfs:label xml:lang="en">was built at time</rdfs:label>
    </owl:ObjectProperty>
    


    <!-- https://w3id.org/polifonia/ontology/instrument/wasBuiltIn -->

    <owl:ObjectProperty rdf:about="https://w3id.org/polifonia/ontology/instrument/wasBuiltIn">
        <rdfs:domain rdf:resource="https://w3id.org/polifonia/ontology/instrument/InstrumentRealization"/>
        <rdfs:range rdf:resource="https://w3id.org/polifonia/ontology/core/Place"/>
        <rdfs:comment xml:lang="en">The relation between an instrument realization and the place it was built in.</rdfs:comment>
        <rdfs:label xml:lang="en">was built in</rdfs:label>
    </owl:ObjectProperty>
    


    <!-- https://w3id.org/polifonia/ontology/instrument/wasInventedAtTime -->

    <owl:ObjectProperty rdf:about="https://w3id.org/polifonia/ontology/instrument/wasInventedAtTime">
        <rdfs:domain rdf:resource="https://w3id.org/polifonia/ontology/instrument/Instrument"/>
        <rdfs:range rdf:resource="https://w3id.org/polifonia/ontology/core/TimeInterval"/>
        <rdfs:comment xml:lang="en">The relation between an instrument, intended as an information object, and the time interval it was invented at.</rdfs:comment>
        <rdfs:label xml:lang="en">was invented at time</rdfs:label>
    </owl:ObjectProperty>
    


    <!-- https://w3id.org/polifonia/ontology/instrument/wasInventedBy -->

    <owl:ObjectProperty rdf:about="https://w3id.org/polifonia/ontology/instrument/wasInventedBy">
        <rdfs:domain rdf:resource="https://w3id.org/polifonia/ontology/instrument/Instrument"/>
        <rdfs:range rdf:resource="https://w3id.org/polifonia/ontology/core/Agent"/>
        <rdfs:comment xml:lang="en">The relation between an instrument as an information object and the agent which invented it.</rdfs:comment>
        <rdfs:label xml:lang="en">was invented by</rdfs:label>
    </owl:ObjectProperty>
    


    <!-- 
    ///////////////////////////////////////////////////////////////////////////////////////
    //
    // Classes
    //
    ///////////////////////////////////////////////////////////////////////////////////////
     -->

    


    <!-- https://w3id.org/polifonia/ontology/instrument/Instrument -->

    <owl:Class rdf:about="https://w3id.org/polifonia/ontology/instrument/Instrument">
        <rdfs:subClassOf rdf:resource="https://w3id.org/polifonia/ontology/core/InformationObject"/>
        <rdfs:subClassOf rdf:resource="https://w3id.org/polifonia/ontology/music-meta/MediumOfPerformance"/>
        <rdfs:subClassOf>
            <owl:Restriction>
                <owl:onProperty rdf:resource="https://w3id.org/polifonia/ontology/instrument/wasInventedAtTime"/>
                <owl:someValuesFrom rdf:resource="https://w3id.org/polifonia/ontology/core/TimeInterval"/>
            </owl:Restriction>
        </rdfs:subClassOf>
        <rdfs:subClassOf>
            <owl:Restriction>
                <owl:onProperty rdf:resource="https://w3id.org/polifonia/ontology/instrument/wasInventedBy"/>
                <owl:someValuesFrom rdf:resource="https://w3id.org/polifonia/ontology/core/Agent"/>
            </owl:Restriction>
        </rdfs:subClassOf>
        <rdfs:subClassOf>
            <owl:Restriction>
                <owl:onProperty rdf:resource="https://w3id.org/arco/ontology/core/hasPart"/>
                <owl:allValuesFrom rdf:resource="https://w3id.org/polifonia/ontology/instrument/InstrumentPart"/>
            </owl:Restriction>
        </rdfs:subClassOf>
        <rdfs:comment xml:lang="en">An instrument intended as an information object (e.g. the guitar as an information object), regardless its physical realizations (e.g. the specific guitar at my place).</rdfs:comment>
        <rdfs:label xml:lang="en">Instrument</rdfs:label>
    </owl:Class>
    


    <!-- https://w3id.org/polifonia/ontology/instrument/InstrumentPart -->

    <owl:Class rdf:about="https://w3id.org/polifonia/ontology/instrument/InstrumentPart">
        <rdfs:comment xml:lang="en">The part of an instrument.</rdfs:comment>
        <rdfs:label xml:lang="en">Instrument part</rdfs:label>
    </owl:Class>
    


    <!-- https://w3id.org/polifonia/ontology/instrument/InstrumentRealization -->

    <owl:Class rdf:about="https://w3id.org/polifonia/ontology/instrument/InstrumentRealization">
        <rdfs:subClassOf rdf:resource="https://w3id.org/polifonia/ontology/core/InformationRealization"/>
        <rdfs:subClassOf>
            <owl:Restriction>
                <owl:onProperty rdf:resource="https://w3id.org/arco/ontology/location/hasTimeIndexedTypedLocation"/>
                <owl:someValuesFrom rdf:resource="https://w3id.org/arco/ontology/location/TimeIndexedTypedLocation"/>
            </owl:Restriction>
        </rdfs:subClassOf>
        <rdfs:subClassOf>
            <owl:Restriction>
                <owl:onProperty rdf:resource="https://w3id.org/polifonia/ontology/core/hasName"/>
                <owl:someValuesFrom rdf:resource="https://w3id.org/polifonia/ontology/core/Name"/>
            </owl:Restriction>
        </rdfs:subClassOf>
        <rdfs:subClassOf>
            <owl:Restriction>
                <owl:onProperty rdf:resource="https://w3id.org/polifonia/ontology/core/realizes"/>
                <owl:someValuesFrom rdf:resource="https://w3id.org/polifonia/ontology/instrument/Instrument"/>
            </owl:Restriction>
        </rdfs:subClassOf>
        <rdfs:subClassOf>
            <owl:Restriction>
                <owl:onProperty rdf:resource="https://w3id.org/polifonia/ontology/instrument/wasBuiltIn"/>
                <owl:someValuesFrom rdf:resource="https://w3id.org/polifonia/ontology/core/Place"/>
            </owl:Restriction>
        </rdfs:subClassOf>
        <rdfs:comment xml:lang="en">The physical realization of an instrument, intended as the information realization (e.g. the specific guitar at my place) and the information object (the guitar as an information object).</rdfs:comment>
        <rdfs:label xml:lang="en">Instrument realization</rdfs:label>
    </owl:Class>
    


    <!-- https://w3id.org/polifonia/ontology/instrument/Voice -->

    <owl:Class rdf:about="https://w3id.org/polifonia/ontology/instrument/Voice">
        <rdfs:subClassOf rdf:resource="https://w3id.org/polifonia/ontology/music-meta/MediumOfPerformance"/>
        <rdfs:label xml:lang="en">Voice</rdfs:label>
    </owl:Class>
</rdf:RDF>



<!-- Generated by the OWL API (version 4.5.9.2019-02-01T07:24:44Z) https://github.com/owlcs/owlapi -->

